% !TeX root = sincotsec.tex

\chapter{Фундаментальные функции}

\section{Определение}

\begin{equation*} \begin{aligned}
&&
&\ldots &
&\ldots \\
%
&&
\elg_{-4}(x) &=
- \frac{3!}{x^4} &
\elh_{-4}(x) &=
- \frac{3!}{x^4} \left(
  \ln{x} - \Theta_3 \right) \\
%
&&
\elg_{-3}(x) &=
  \frac{2!}{x^3} &
\elh_{-3}(x) &=
  \frac{2!}{x^3} \left(
  \ln{x} - \Theta_2 \right) \\
%
&& 
\elg_{-2}(x) &=
- \frac{1!}{x^2} &
\elh_{-2}(x) &=
- \frac{1!}{x^2} \left(
  \ln{x} - \Theta_1 \right) \\
%
&& 
\elg_{-1}(x) &=
  \frac{0!}{x^1} &
\elh_{-1}(x) &=
  \frac{0!}{x^1} \left(
  \ln{x} - \Theta_0 \right) \\
%
\elf_0(x) &=
  \frac{x^0}{0!} &
\elg_0(x) &= 
  \frac{x^0}{0!} \left(
  \ln{x} - \Theta_0 \right) &
\elh_0(x) &=
  \frac{x^0}{0!} \left(
  \frac{\ln^2{x}}{2}
- \Theta_0 \ln{x}
+ \Lambda_0 \right) \\
%
\elf_1(x) &=
  \frac{x^1}{1!} &
\elg_1(x) &= 
  \frac{x^1}{1!} \left(
  \ln{x} - \Theta_1 \right) &
\elh_1(x) &=
  \frac{x^1}{1!} \left(
  \frac{\ln^2{x}}{2}
- \Theta_1 \ln{x}
+ \Lambda_1 \right) \\
%
\elf_2(x) &=
  \frac{x^2}{2!} &
\elg_2(x) &= 
  \frac{x^2}{2!} \left(
  \ln{x} - \Theta_2 \right) &
\elh_2(x) &=
  \frac{x^2}{2!} \left(
  \frac{\ln^2{x}}{2}
- \Theta_2 \ln{x}
+ \Lambda_2 \right) \\
%
\elf_3(x) &=
  \frac{x^3}{3!} &
\elg_3(x) &= 
  \frac{x^3}{3!} \left(
  \ln{x} - \Theta_3 \right) &
\elh_3(x) &=
  \frac{x^3}{3!} \left(
  \frac{\ln^2{x}}{2}
- \Theta_3 \ln{x}
+ \Lambda_3 \right) \\
%
\elf_4(x) &=
  \frac{x^4}{4!} &
\elg_4(x) &= 
  \frac{x^4}{4!} \left(
  \ln{x} - \Theta_4 \right) &
\elh_4(x) &=
  \frac{x^4}{4!} \left(
  \frac{\ln^2{x}}{2}
- \Theta_4 \ln{x}
+ \Lambda_4 \right) \\
%
&\ldots &
&\ldots &
&\ldots \\
\end{aligned} \end{equation*}
%%
\begin{equation*} \begin{aligned}
\Theta_0 &= 0 &
\Lambda_0 &= 0 \\
%
\Theta_1 &= 
  \frac{1}{1} &
\Lambda_1 &= 
  \frac{1}{1^2} \\
%
\Theta_2 &= 
  \frac{1}{1} 
+ \frac{1}{2} &
\Lambda_2 &= 
  \frac{1}{1^2} 
+ \frac{1}{1 \cdot 2} 
+ \frac{1}{2^2} \\
%
\Theta_3 &= 
  \frac{1}{1} 
+ \frac{1}{2} 
+ \frac{1}{3} &
\Lambda_3 &= 
  \frac{1}{1^2} 
+ \frac{1}{1 \cdot 2} 
+ \frac{1}{2^2}
+ \frac{1}{1 \cdot 3}
+ \frac{1}{2 \cdot 3}
+ \frac{1}{3^2} \\
%
\Theta_4 &= 
  \frac{1}{1} 
+ \frac{1}{2} 
+ \frac{1}{3} 
+ \frac{1}{4} &
\Lambda_4 &= 
  \frac{1}{1^2} 
+ \frac{1}{1 \cdot 2} 
+ \frac{1}{2^2}
+ \frac{1}{1 \cdot 3}
+ \frac{1}{2 \cdot 3}
+ \frac{1}{3^2}
+ \frac{1}{1 \cdot 4}
+ \frac{1}{2 \cdot 4}
+ \frac{1}{3 \cdot 4}
+ \frac{1}{4^2} \\
%
&\ldots & &\ldots \\
\end{aligned} \end{equation*}

\begin{equation*} \begin{aligned}
\mathrm{D}_1 \elf_n(x) &= \elf_{n - 1}(x) \\
\mathrm{D}_1 \elg_n(x) &= \elg_{n - 1}(x) \\
\mathrm{D}_1 \elh_n(x) &= \elh_{n - 1}(x) \\
\end{aligned} \end{equation*}