% !TeX root = sincotsec.tex

\subsection{Натуральные корни}

\begin{equation*} \begin{aligned}
A(x) &=
\frac{1}
{
  \left(1 + \displaystyle \frac{x}{1} \right)
  \left(1 + \displaystyle \frac{x}{2} \right)
  \left(1 + \displaystyle \frac{x}{3} \right)
  \cdot \ldots \cdot
  \left(1 + \displaystyle \frac{x}{n} \right)
} &
= \frac{\theta_1}{1 + \cfrac{x}{1}}
+ \frac{\theta_2}{1 + \cfrac{x}{2}}
+ \frac{\theta_3}{1 + \cfrac{x}{3}}
+ \ldots
+ \frac{\theta_n}{1 + \cfrac{x}{n}} \\
\end{aligned} \end{equation*}

\begin{equation*} \begin{aligned}
\theta_1 &= \frac{1}
{
  \left(1 - \displaystyle \frac{1}{2} \right)
  \left(1 - \displaystyle \frac{1}{3} \right)
  \cdot \ldots \cdot
  \left(1 - \displaystyle \frac{1}{n - 1} \right)
  \left(1 - \displaystyle \frac{1}{n} \right)
} \\
\theta_2 &= \frac{1}
{
  \left(1 - \displaystyle \frac{2}{1} \right)
  \left(1 - \displaystyle \frac{2}{3} \right)
  \cdot \ldots \cdot
  \left(1 - \displaystyle \frac{2}{n - 1} \right)
  \left(1 - \displaystyle \frac{2}{n} \right)
} \\
\theta_3 &= \frac{1}
{
  \left(1 - \displaystyle \frac{3}{1} \right)
  \left(1 - \displaystyle \frac{3}{2} \right)
  \cdot \ldots \cdot
  \left(1 - \displaystyle \frac{3}{n - 1} \right)
  \left(1 - \displaystyle \frac{3}{n} \right)
} \\
&\ldots \\
\theta_n &= \frac{1}
{
  \left(1 - \displaystyle \frac{n}{1} \right)
  \left(1 - \displaystyle \frac{n}{2} \right)
  \left(1 - \displaystyle \frac{n}{3} \right)
  \cdot \ldots \cdot
  \left(1 - \displaystyle \frac{n}{n - 1} \right)
} \\
\end{aligned} \end{equation*}

\begin{equation*} \left| \begin{aligned}
A(x) = \Psi(x) &=
  \psi_0 x^0 
+ \psi_1 x^1
+ \psi_2 x^2 
+ \psi_3 x^3 
+ \ldots &
&|x| < |c_1| \\
%
A(x) = S_1(x) &= 
  t_{(1,-1)} x^{-1}
+ t_{(1,-2)} x^{-2}
+ t_{(1,-3)} x^{-3}
+ \ldots \\ &
+ s_{(1,0)} x^0
+ s_{(1,1)} x^1
+ s_{(1,2)} x^2
+ s_{(1,3)} x^3
+ \ldots &
|c_1| < &|x| < |c_2| \\
%
A(x) = S_2(x) &= 
  t_{(2,-1)} x^{-1}
+ t_{(2,-2)} x^{-2}
+ t_{(2,-3)} x^{-3}
+ \ldots \\ &
+ s_{(2,0)} x^0
+ s_{(2,1)} x^1
+ s_{(2,2)} x^2
+ s_{(2,3)} x^3
+ \ldots &
|c_2| < &|x| < |c_3| \\
%
A(x) = S_3(x) &= 
  t_{(3,-1)} x^{-1}
+ t_{(3,-2)} x^{-2}
+ t_{(3,-3)} x^{-3}
+ \ldots \\ &
+ s_{(3,0)} x^0
+ s_{(3,1)} x^1
+ s_{(3,2)} x^2
+ s_{(3,3)} x^3
+ \ldots &
|c_3| < &|x| < |c_4| \\
%
&\ldots \\
%
A(x) = S_n(x) &= 
  t_{(n,-1)} x^{-1}
+ t_{(n,-2)} x^{-2}
+ t_{(n,-3)} x^{-3}
+ \ldots \\ &
+ s_{(n,0)} x^0
+ s_{(n,1)} x^1
+ s_{(n,2)} x^2
+ s_{(n,3)} x^3
+ \ldots &
|c_n| < &|x| \\
\end{aligned} \right. \end{equation*}

\begin{equation*} \left| \begin{aligned}
\psi_0 &= \left(
  \frac{\theta_1}{1^0}
+ \frac{\theta_2}{2^0}
+ \frac{\theta_3}{3^0}
+ \ldots
+ \frac{\theta_n}{n^0} \right) \\
%
\psi_1 &= - \left(
  \frac{\theta_1}{1^1}
+ \frac{\theta_2}{2^1}
+ \frac{\theta_3}{3^1}
+ \ldots
+ \frac{\theta_n}{n^1} \right) \\
%
\psi_2 &= \left(
  \frac{\theta_1}{1^2}
+ \frac{\theta_2}{2^2}
+ \frac{\theta_3}{3^2}
+ \ldots
+ \frac{\theta_n}{n^2} \right) \\
%
\psi_3 &= - \left(
  \frac{\theta_1}{1^3}
+ \frac{\theta_2}{2^3}
+ \frac{\theta_3}{3^3}
+ \ldots
+ \frac{\theta_n}{n^3} \right) \\
%
&\ldots \\
\end{aligned} \right. \end{equation*}

\begin{equation*} \left| \begin{aligned}
t_{(1,-1)} &=
  \frac{\theta_1}{1^{-1}} \\
%
t_{(1,-2)} &=
  - \frac{\theta_1}{1^{-2}} \\
%
t_{(1,-3)} &=
  \frac{\theta_1}{1^{-3}} \\
%
&\ldots \\
%
s_{(1,0)} &=
- \frac{\theta_1}{1^0}
+ \psi_0 \\
%
s_{(1,1)} &=
  \frac{\theta_1}{1^1}
+ \psi_1 \\
%
s_{(1,2)} &=
- \frac{\theta_1}{1^2}
+ \psi_2 \\
%
s_{(1,3)} &=
  \frac{\theta_1}{1^3}
+ \psi_3 \\
%
&\ldots \\
\end{aligned} \right. \end{equation*}

\begin{equation*} \left| \begin{aligned}
t_{(2,-1)} &=
  \left(
  \frac{\theta_1}{1^{-1}}
+ \frac{\theta_2}{2^{-1}} \right) \\
%
t_{(2,-2)} &=
- \left(
  \frac{\theta_1}{1^{-2}}
+ \frac{\theta_2}{2^{-2}} \right) \\
%
t_{(2,-3)} &=
  \left(
  \frac{\theta_1}{1^{-3}}
+ \frac{\theta_2}{2^{-3}} \right) \\
%
&\ldots \\
%
s_{(2,0)} &=
- \left(
  \frac{\theta_1}{1^0}
+ \frac{\theta_2}{2^0} \right)
+ \psi_0 \\
%
s_{(2,1)} &=
  \left(
  \frac{\theta_1}{1^1}
+ \frac{\theta_2}{2^1} \right)
+ \psi_1 \\
%
s_{(2,2)} &=
- \left(
  \frac{\theta_1}{1^2}
+ \frac{\theta_2}{2^2} \right)
+ \psi_2 \\
%
s_{(2,3)} &=
  \left(
  \frac{\theta_1}{1^3}
+ \frac{\theta_2}{2^3} \right)
+ \psi_3 \\
%
&\ldots \\
\end{aligned} \right. \end{equation*}

\begin{equation*} \left| \begin{aligned}
t_{(3,-1)} &=
  \left(
  \frac{\theta_1}{1^{-1}}
+ \frac{\theta_2}{2^{-1}}
+ \frac{\theta_3}{3^{-1}} \right) \\
%
t_{(3,-2)} &=
- \left(
  \frac{\theta_1}{1^{-2}}
+ \frac{\theta_2}{2^{-2}}
+ \frac{\theta_3}{3^{-2}} \right) \\
%
t_{(3,-3)} &=
  \left(
  \frac{\theta_1}{1^{-3}}
+ \frac{\theta_2}{2^{-3}}
+ \frac{\theta_3}{3^{-3}} \right) \\
%
&\ldots \\
%
s_{(3,0)} &=
- \left(
  \frac{\theta_1}{1^0}
+ \frac{\theta_2}{2^0}
+ \frac{\theta_3}{3^0} \right)
+ \psi_0 \\
%
s_{(3,1)} &=
  \left(
  \frac{\theta_1}{1^1}
+ \frac{\theta_2}{2^1}
+ \frac{\theta_3}{3^1} \right)
+ \psi_1 \\
%
s_{(3,2)} &=
- \left(
  \frac{\theta_1}{1^2}
+ \frac{\theta_2}{2^2}
+ \frac{\theta_3}{3^2} \right)
+ \psi_2 \\
%
s_{(3,3)} &=
  \left(
  \frac{\theta_1}{1^3}
+ \frac{\theta_2}{2^3}
+ \frac{\theta_3}{3^3} \right)
+ \psi_3 \\
%
&\ldots \\
\end{aligned} \right. \end{equation*}

\begin{equation*} \left| \begin{aligned}
t_{(n,-1)} &=
  \left(
  \frac{\theta_1}{1^{-1}}
+ \frac{\theta_2}{2^{-1}}
+ \frac{\theta_3}{3^{-1}}
+ \ldots
+ \frac{\theta_n}{n^{-1}} \right) \\
%
t_{(n,-2)} &=
- \left(
  \frac{\theta_1}{1^{-2}}
+ \frac{\theta_2}{2^{-2}}
+ \frac{\theta_3}{3^{-2}}
+ \ldots
+ \frac{\theta_n}{n^{-2}} \right) \\
%
t_{(n,-3)} &=
  \left(
  \frac{\theta_1}{1^{-3}}
+ \frac{\theta_2}{2^{-3}}
+ \frac{\theta_3}{3^{-3}}
+ \ldots
+ \frac{\theta_n}{n^{-3}} \right) \\
%
&\ldots \\
%
s_{(n,0)} &=
- \left(
  \frac{\theta_1}{1^0}
+ \frac{\theta_2}{2^0}
+ \frac{\theta_3}{3^0}
+ \ldots
+ \frac{\theta_n}{n^0} \right)
+ \psi_0 \\
%
s_{(n,1)} &=
  \left(
  \frac{\theta_1}{1^1}
+ \frac{\theta_2}{2^1}
+ \frac{\theta_3}{3^1}
+ \ldots
+ \frac{\theta_n}{n^1} \right)
+ \psi_1 \\
%
s_{(n,2)} &=
- \left(
  \frac{\theta_1}{1^2}
+ \frac{\theta_2}{2^2}
+ \frac{\theta_3}{3^2}
+ \ldots
+ \frac{\theta_n}{n^2} \right)
+ \psi_2 \\
%
s_{(n,3)} &=
  \left(
  \frac{\theta_1}{1^3}
+ \frac{\theta_2}{2^3}
+ \frac{\theta_3}{3^3}
+ \ldots
+ \frac{\theta_n}{n^3} \right)
+ \psi_3 \\
%
&\ldots \\
\end{aligned} \right. \end{equation*}