% !TeX root = sincotsec.tex

\subsection{Корни -- все целые числа без нуля}

\begin{equation*} \begin{aligned}
A(x) &=
  \ln{\left(1 + \frac{x}{1} \right)}
+ \ln{\left(1 + \frac{x}{2} \right)}
+ \ln{\left(1 + \frac{x}{3} \right)}
+ \ldots \\ &
+ \ln{\left(1 - \frac{x}{1} \right)}
+ \ln{\left(1 - \frac{x}{2} \right)}
+ \ln{\left(1 - \frac{x}{3} \right)}
+ \ldots
\end{aligned} \end{equation*}

\begin{equation*} \left| \begin{aligned}
A(x) = \Psi(x) &=
  \psi_0 x^0
+ \psi_2 x^2
+ \psi_4 x^4
+ \psi_6 x^6
+ \ldots &
&|x| < 1 \\
%
A(x) = S_1(x) &= 
  t_{(1,0)} x^0 \ln{x}
+ t_{(1,-2)} x^{-2}
+ t_{(1,-4)} x^{-4}
+ t_{(1,-6)} x^{-6}
+ \ldots \\ &
+ s_{(1,0)} x^0
+ s_{(1,2)} x^2
+ s_{(1,4)} x^4
+ s_{(1,6)} x^6
+ \ldots &
1 < &|x| < 2 \\
%
A(x) = S_2(x) &= 
  t_{(2,0)} x^0 \ln{x}
+ t_{(2,-2)} x^{-2}
+ t_{(2,-4)} x^{-4}
+ t_{(2,-6)} x^{-6}
+ \ldots \\ &
+ s_{(2,0)} x^0
+ s_{(2,2)} x^2
+ s_{(2,4)} x^4
+ s_{(2,6)} x^6
+ \ldots &
2 < &|x| < 3 \\
%
A(x) = S_3(x) &= 
  t_{(3,0)} x^0 \ln{x}
+ t_{(3,-2)} x^{-2}
+ t_{(3,-4)} x^{-4}
+ t_{(3,-6)} x^{-6}
+ \ldots \\ &
+ s_{(3,0)} x^0
+ s_{(3,2)} x^2
+ s_{(3,4)} x^4
+ s_{(3,6)} x^6
+ \ldots &
3 < &|x| < 4 \\
%
&\ldots \\
%
A(x) = S_n(x) &= 
  t_{(n,0)} x^0 \ln{x}
+ t_{(n,-2)} x^{-2}
+ t_{(n,-4)} x^{-4}
+ t_{(n,-6)} x^{-6}
+ \ldots \\ &
+ s_{(n,0)} x^0
+ s_{(n,2)} x^2
+ s_{(n,4)} x^4
+ s_{(n,6)} x^6
+ \ldots &
n < &|x| \\
\end{aligned} \right. \end{equation*}

\begin{equation*} \left| \begin{aligned}
\psi_0 &= 2 \ln{1}
  \left(
  \frac{1}{1^0}
+ \frac{1}{2^0}
+ \frac{1}{3^0}
+ \ldots
  \right) \\
%
\psi_2 &=
- \frac{2}{2}
  \left(
  \frac{1}{1^2}
+ \frac{1}{2^2}
+ \frac{1}{3^2}
+ \ldots
  \right) \\
%
\psi_4 &=
- \frac{2}{4}
  \left(
  \frac{1}{1^4}
+ \frac{1}{2^4}
+ \frac{1}{3^4}
+ \ldots
  \right) \\
%
\psi_6 &=
- \frac{2}{6}
  \left(
  \frac{1}{1^6}
+ \frac{1}{2^6}
+ \frac{1}{3^6}
+ \ldots
  \right) \\
%
&\ldots \\
\end{aligned} \right. \end{equation*}

\begin{equation*} \left| \begin{aligned}
t_{(1,0)} &=
  2 \frac{1}{1^0} \\
%
t_{(1,-2)} &=
- \frac{2}{2}
  \frac{1}{1^{-2}} \\
%
t_{(1,-4)} &=
- \frac{2}{4}
  \frac{1}{1^{-4}} \\
%
t_{(1,-6)} &=
- \frac{2}{6}
  \frac{1}{1^{-6}} \\
&\ldots \\
%
s_{(1,0)} &=
- 2 \ln{1}
  \frac{1}{1^0}
- \frac{\ln{(- 1^2)}}{1^0}
+ \psi_0 \\
%
s_{(1,2)} &=
  \frac{2}{2}
  \frac{1}{1^2}
+ \psi_2 \\
%
s_{(1,4)} &=
  \frac{2}{4}
  \frac{1}{1^4}
+ \psi_4 \\
%
s_{(1,6)} &=
  \frac{2}{6}
  \frac{1}{1^6}
+ \psi_6 \\
%
&\ldots \\
\end{aligned} \right. \end{equation*}

\begin{equation*} \left| \begin{aligned}
t_{(2,0)} &=
  2
  \left(
  \frac{1}{1^0}
+ \frac{1}{2^0}
  \right) \\
%
t_{(2,-2)} &=
- \frac{2}{2}
  \left(
  \frac{1}{1^{-2}}
+ \frac{1}{2^{-2}}
  \right) \\
%
t_{(2,-4)} &=
- \frac{2}{4}
  \left(
  \frac{1}{1^{-4}}
+ \frac{1}{2^{-4}}
  \right) \\
%
t_{(2,-6)} &=
- \frac{2}{6}
  \left(
  \frac{1}{1^{-6}}
+ \frac{1}{2^{-6}}
  \right) \\
%
&\ldots \\
%
s_{(2,0)} &=
- 2 \ln{1}
  \left(
  \frac{1}{1^0}
+ \frac{1}{2^0}
  \right)
- \left(
  \frac{\ln{(- 1^2)}}{1^0}
+ \frac{\ln{(- 2^2)}}{2^0}
  \right)
+ \psi_0 \\
%
s_{(2,2)} &=
  \frac{2}{2}
  \left(
  \frac{1}{1^2}
+ \frac{1}{2^2}
  \right)
+ \psi_2 \\
%
s_{(2,4)} &=
  \frac{2}{4}
  \left(
  \frac{1}{1^4}
+ \frac{1}{2^4}
  \right)
+ \psi_4 \\
%
s_{(2,6)} &=
  \frac{2}{6}
  \left(
  \frac{1}{1^6}
+ \frac{1}{2^6}
  \right)
+ \psi_6 \\
%
&\ldots \\
\end{aligned} \right. \end{equation*}

\begin{equation*} \left| \begin{aligned}
t_{(3,0)} &=
  2
  \left(
  \frac{1}{1^0}
+ \frac{1}{2^0}
+ \frac{1}{3^0}
  \right) \\
%
t_{(3,-2)} &=
- \frac{2}{2}
  \left(
  \frac{1}{1^{-2}}
+ \frac{1}{2^{-2}}
+ \frac{1}{3^{-2}}
  \right) \\
%
t_{(3,-4)} &=
- \frac{2}{4}
  \left(
  \frac{1}{1^{-4}}
+ \frac{1}{2^{-4}}
+ \frac{1}{3^{-4}}
  \right) \\
%
t_{(3,-6)} &=
- \frac{2}{6}
  \left(
  \frac{1}{1^{-6}}
+ \frac{1}{2^{-6}}
+ \frac{1}{3^{-6}}
  \right) \\
%
&\ldots \\
%
s_{(3,0)} &=
- 2 \ln{1}
  \left(
  \frac{1}{1^0}
+ \frac{1}{2^0}
+ \frac{1}{3^0}
  \right)
- \left(
  \frac{\ln{(- 1^2)}}{1^0}
+ \frac{\ln{(- 2^2)}}{2^0}
+ \frac{\ln{(- 3^2)}}{3^0}
  \right)
+ \psi_0 \\
%
s_{(3,2)} &=
  \frac{2}{2}
  \left(
  \frac{1}{1^2}
+ \frac{1}{2^2}
+ \frac{1}{3^2}
  \right)
+ \psi_2 \\
%
s_{(3,4)} &=
  \frac{2}{4}
  \left(
  \frac{1}{1^4}
+ \frac{1}{2^4}
+ \frac{1}{3^4}
  \right)
+ \psi_4 \\
%
s_{(3,6)} &=
  \frac{2}{6}
  \left(
  \frac{1}{1^6}
+ \frac{1}{2^6}
+ \frac{1}{3^6}
  \right)
+ \psi_6 \\
%
&\ldots \\
\end{aligned} \right. \end{equation*}