% !TeX root = sincotsec.tex

\subsection{Натуральные корни}

\begin{equation*} \begin{aligned}
&A(x) =
  \ln{\left(1 + \frac{x}{1} \right)}
+ \ln{\left(1 + \frac{x}{2} \right)}
+ \ln{\left(1 + \frac{x}{3} \right)}
+ \ldots
+ \ln{\left(1 + \frac{x}{n} \right)}
\end{aligned} \end{equation*}

\begin{equation*} \left| \begin{aligned}
A(x) = \Psi(x) &=
  \psi_0 x^0
+ \psi_1 x^1
+ \psi_2 x^2
+ \psi_3 x^3
+ \ldots &
&|x| < 1 \\
%
A(x) = S_1(x) &= 
  t_{(1,0)} x^0 \ln{x}
+ t_{(1,-1)} x^{-1}
+ t_{(1,-2)} x^{-2}
+ t_{(1,-3)} x^{-3}
+ \ldots \\ &
+ s_{(1,0)} x^0
+ s_{(1,1)} x^1
+ s_{(1,2)} x^2
+ s_{(1,3)} x^3
+ \ldots &
1 < &|x| < 2 \\
%
A(x) = S_2(x) &= 
  t_{(2,0)} x^0 \ln{x}
+ t_{(2,-1)} x^{-1}
+ t_{(2,-2)} x^{-2}
+ t_{(2,-3)} x^{-3}
+ \ldots \\ &
+ s_{(2,0)} x^0
+ s_{(2,1)} x^1
+ s_{(2,2)} x^2
+ s_{(2,3)} x^3
+ \ldots &
2 < &|x| < 3 \\
%
A(x) = S_3(x) &= 
  t_{(3,0)} x^0 \ln{x}
+ t_{(3,-1)} x^{-1}
+ t_{(3,-2)} x^{-2}
+ t_{(3,-3)} x^{-3}
+ \ldots \\ &
+ s_{(3,0)} x^0
+ s_{(3,1)} x^1
+ s_{(3,2)} x^2
+ s_{(3,3)} x^3
+ \ldots &
3 < &|x| < 4 \\
%
&\ldots \\
%
A(x) = S_n(x) &= 
  t_{(n,0)} x^0 \ln{x}
+ t_{(n,-1)} x^{-1}
+ t_{(n,-2)} x^{-2}
+ t_{(n,-3)} x^{-3}
+ \ldots \\ &
+ s_{(n,0)} x^0
+ s_{(n,1)} x^1
+ s_{(n,2)} x^2
+ s_{(n,3)} x^3
+ \ldots &
n < &|x| \\
\end{aligned} \right. \end{equation*}

\begin{equation*} \left| \begin{aligned}
\psi_0 &= \ln{1} \left(
  \frac{1}{1^0}
+ \frac{1}{2^0}
+ \frac{1}{3^0}
+ \ldots
+ \frac{1}{n^0} \right) \\
%
\psi_1 &= \frac{1}{1} \left(
  \frac{1}{1^1}
+ \frac{1}{2^1}
+ \frac{1}{3^1}
+ \ldots
+ \frac{1}{n^1} \right) \\
%
\psi_2 &= - \frac{1}{2} \left(
  \frac{1}{1^2}
+ \frac{1}{2^2}
+ \frac{1}{3^2}
+ \ldots
+ \frac{1}{n^2} \right) \\
%
\psi_3 &= \frac{1}{3} \left(
  \frac{1}{1^3}
+ \frac{1}{2^3}
+ \frac{1}{3^3}
+ \ldots
+ \frac{1}{n^3} \right) \\
%
&\ldots \\
\end{aligned} \right. \end{equation*}

\begin{equation*} \left| \begin{aligned}
t_{(1,0)} &=
  \frac{1}{1^0} \\
%
t_{(1,-1)} &=
  \frac{1}{1} \frac{1}{1^{-1}} \\
%
t_{(1,-2)} &=
  - \frac{1}{2} \frac{1}{1^{-2}} \\
%
t_{(1,-3)} &=
  \frac{1}{3} \frac{1}{1^{-3}} \\
%
&\ldots \\
%
s_{(1,0)} &=
- \ln{1} \frac{1}{1^0}
- \frac{\ln{1}}{1^0}
+ \psi_0 \\
%
s_{(1,1)} &=
- \frac{1}{1} \frac{1}{1^1}
+ \psi_1 \\
%
s_{(1,2)} &=
  \frac{1}{2} \frac{1}{1^2}
+ \psi_2 \\
%
s_{(1,3)} &=
- \frac{1}{3} \frac{1}{1^3}
+ \psi_3 \\
%
&\ldots \\
\end{aligned} \right. \end{equation*}

\begin{equation*} \left| \begin{aligned}
t_{(2,0)} &=
  \left(
  \frac{1}{1^0}
+ \frac{1}{2^0} \right) \\
%
t_{(2,-1)} &=
  \frac{1}{1} \left(
  \frac{1}{1^{-1}}
+ \frac{1}{2^{-1}} \right) \\
%
t_{(2,-2)} &=
- \frac{1}{2} \left(
  \frac{1}{1^{-2}}
+ \frac{1}{2^{-2}} \right) \\
%
t_{(2,-3)} &=
  \frac{1}{3} \left(
  \frac{1}{1^{-3}}
+ \frac{1}{2^{-3}} \right) \\
%
&\ldots \\
%
s_{(2,0)} &=
- \ln{1} \left(
  \frac{1}{1^0}
+ \frac{1}{2^0} \right)
- \left(
  \frac{\ln{1}}{1^0}
+ \frac{\ln{2}}{2^0} \right)
+ \psi_0 \\
%
s_{(2,1)} &=
- \frac{1}{1} \left(
  \frac{1}{1^1}
+ \frac{1}{2^1} \right)
+ \psi_1 \\
%
s_{(2,2)} &=
  \frac{1}{2} \left(
  \frac{1}{1^2}
+ \frac{1}{2^2} \right)
+ \psi_2 \\
%
s_{(2,3)} &=
- \frac{1}{3} \left(
  \frac{1}{1^3}
+ \frac{1}{2^3} \right)
+ \psi_3 \\
%
&\ldots \\
\end{aligned} \right. \end{equation*}

\begin{equation*} \left| \begin{aligned}
t_{(3,0)} &=
  \left(
  \frac{1}{1^0}
+ \frac{1}{2^0}
+ \frac{1}{3^0} \right) \\
%
t_{(3,-1)} &=
  \frac{1}{1} \left(
  \frac{1}{1^{-1}}
+ \frac{1}{2^{-1}}
+ \frac{1}{3^{-1}} \right) \\
%
t_{(3,-2)} &=
- \frac{1}{2} \left(
  \frac{1}{1^{-2}}
+ \frac{1}{2^{-2}}
+ \frac{1}{3^{-2}} \right) \\
%
t_{(3,-3)} &=
  \frac{1}{3} \left(
  \frac{1}{1^{-3}}
+ \frac{1}{2^{-3}}
+ \frac{1}{3^{-3}} \right) \\
%
&\ldots \\
%
s_{(3,0)} &=
- \ln{1} \left(
  \frac{1}{1^0}
+ \frac{1}{2^0}
+ \frac{1}{3^0} \right)
- \left(
  \frac{\ln{1}}{1^0}
+ \frac{\ln{2}}{2^0}
+ \frac{\ln{3}}{3^0} \right)
+ \psi_0 \\
%
s_{(3,1)} &=
- \frac{1}{1} \left(
  \frac{1}{1^1}
+ \frac{1}{2^1}
+ \frac{1}{3^1} \right)
+ \psi_1 \\
%
s_{(3,2)} &=
  \frac{1}{2} \left(
  \frac{1}{1^2}
+ \frac{1}{2^2}
+ \frac{1}{3^2} \right)
+ \psi_2 \\
%
s_{(3,3)} &=
- \frac{1}{3} \left(
  \frac{1}{1^3}
+ \frac{1}{2^3}
+ \frac{1}{3^3} \right)
+ \psi_3 \\
%
&\ldots \\
\end{aligned} \right. \end{equation*}

\begin{equation*} \left| \begin{aligned}
t_{(n,0)} &=
  \left(
  \frac{1}{1^0}
+ \frac{1}{2^0}
+ \frac{1}{3^0}
+ \ldots
+ \frac{1}{n^0} \right) \\
%
t_{(n,-1)} &=
  \frac{1}{1} \left(
  \frac{1}{1^{-1}}
+ \frac{1}{2^{-1}}
+ \frac{1}{3^{-1}}
+ \ldots
+ \frac{1}{n^{-1}} \right) \\
%
t_{(n,-2)} &=
- \frac{1}{2} \left(
  \frac{1}{1^{-2}}
+ \frac{1}{2^{-2}}
+ \frac{1}{3^{-2}}
+ \ldots
+ \frac{1}{n^{-2}} \right) \\
%
t_{(n,-3)} &=
  \frac{1}{3} \left(
  \frac{1}{1^{-3}}
+ \frac{1}{2^{-3}}
+ \frac{1}{3^{-3}}
+ \ldots
+ \frac{1}{n^{-3}} \right) \\
%
&\ldots \\
%
s_{(n,0)} &=
- \ln{1} \left(
  \frac{1}{1^0}
+ \frac{1}{2^0}
+ \frac{1}{3^0}
+ \ldots
+ \frac{1}{n^0} \right)
- \left(
  \frac{\ln{1}}{1^0}
+ \frac{\ln{2}}{2^0}
+ \frac{\ln{3}}{3^0}
+ \ldots
+ \frac{\ln{n}}{n^0} \right)
+ \psi_0 \\
%
s_{(n,1)} &=
- \frac{1}{1} \left(
  \frac{1}{1^1}
+ \frac{1}{2^1}
+ \frac{1}{3^1}
+ \ldots
+ \frac{1}{n^1} \right)
+ \psi_1 \\
%
s_{(n,2)} &=
  \frac{1}{2} \left(
  \frac{1}{1^2}
+ \frac{1}{2^2}
+ \frac{1}{3^2}
+ \ldots
+ \frac{1}{n^2} \right)
+ \psi_2 \\
%
s_{(n,3)} &=
- \frac{1}{3} \left(
  \frac{1}{1^3}
+ \frac{1}{2^3}
+ \frac{1}{3^3}
+ \ldots
+ \frac{1}{n^3} \right)
+ \psi_3 \\
%
&\ldots \\
\end{aligned} \right. \end{equation*}