% !TeX root = sincotsec.tex

\subsection{Симметричные натуральные корни}

\begin{equation*} \begin{aligned}
B(x) &= \frac{1}{
\left(1 - \displaystyle \frac{x^2}{1^2} \right)
\left(1 - \displaystyle \frac{x^2}{2^2} \right)
\left(1 - \displaystyle \frac{x^2}{3^2} \right) \cdot
\ldots \cdot
\left(1 - \displaystyle \frac{x^2}{n^2} \right)
} \\ &
= \frac{b_1}{1 - \cfrac{x^2}{1^2}}
+ \frac{b_2}{1 - \cfrac{x^2}{2^2}}
+ \frac{b_3}{1 - \cfrac{x^2}{3^2}}
+ \ldots
+ \frac{b_n}{1 - \cfrac{x^2}{n^2}} \\
\end{aligned} \end{equation*}

\begin{equation*} \begin{aligned}
b_1 &=
  2
  \frac{n}{n + 1}
  \\
b_2 &=
  - 2
  \frac{n}{n + 1}
  \frac{n - 1}{n + 2}
  \\
b_3 &=
  2
  \frac{n}{n + 1}
  \frac{n - 1}{n + 2}
  \frac{n - 2}{n + 3}
  \\
&\ldots
  \\
b_n &=
  - (-1)^n 2
  \frac{n}{n + 1}
  \frac{n - 1}{n + 2}
  \frac{n - 2}{n + 3}
  \cdot
  \ldots
  \cdot
  \frac{1}{2 n}
  \\
\end{aligned} \end{equation*}

\begin{equation*} \left| \begin{aligned}
B(x) = \Xi(x) &=
  \xi_0 \elf_0(x)
+ \xi_2 \elf_2(x)  
+ \ldots & 
&|x| < 1 \\
%
B(x) = H_1(x) &= 
  h_{(1,-2)} \elg_{-2}(x)
+ h_{(1,-4)} \elg_{-4}(x)
+ \ldots \\ &
+ j_{(1,0)} \elf_0(x)
+ j_{(1,2)} \elf_2(x)
+ \ldots & 
1 < &|x| < 2 \\
%
B(x) = H_2(x) &=
  h_{(2,-2)} \elg_{-2}(x)
+ h_{(2,-4)} \elg_{-4}(x)
+ \ldots \\ &
+ j_{(2,0)} \elf_0(x)
+ j_{(2,2)} \elf_2(x)
+ \ldots & 
2 < &|x| < 3 \\
%
B(x) = H_3(x) &=
  h_{(3,-2)} \elg_{-2}(x)
+ h_{(3,-4)} \elg_{-4}(x)
+ \ldots \\ &
+ j_{(3,0)} \elf_0(x)
+ j_{(3,2)} \elf_2(x)
+ \ldots &
3 < &|x| < 4 \\
%
&\ldots & & \\
%
B(x) = H_n(x) &=
  h_{(n,-2)} \elg_{-2}(x)
+ h_{(n,-4)} \elg_{-4}(x)
+ \ldots \\ &
+ j_{(n,0)} \elf_0(x)
+ j_{(n,2)} \elf_2(x)
+ \ldots &
n < &|x| \\
\end{aligned} \right. \end{equation*}

\begin{equation*} \left| \begin{aligned}
\xi_0 &= \elg_{-1}(1) \left(
  \frac{b_1}{1^0}
+ \frac{b_2}{2^0}
+ \frac{b_3}{3^0}
+ \ldots
+ \frac{b_n}{n^0} \right) \\
%
\xi_2 &= \elg_{-3}(1) \left(
  \frac{b_1}{1^2}
+ \frac{b_2}{2^2}
+ \frac{b_3}{3^2}
+ \ldots
+ \frac{b_n}{n^2} \right) \\
%
&\ldots \\
\end{aligned} \right. \end{equation*}
%
\begin{equation*} \left| \begin{aligned}
%
h_{(1,-2)} &=
  \elf_1(1) \frac{b_1}{1^{-2}} \\
%
h_{(1,-4)} &=
  \elf_3(1) \frac{b_1}{1^{-4}} \\
%
&\ldots \\
%
j_{(1,0)} &=
- \elg_{-1}(1) \frac{b_1}{1^0}
+ \xi_0 \\
%
j_{(1,2)} &=
- \elg_{-3}(1) \frac{b_1}{1^2}
+ \xi_2 \\
%
&\ldots \\
\end{aligned} \right. \end{equation*}

\begin{equation*} \left| \begin{aligned}
h_{(2,-2)} &=
  \elf_1(1) \left(
  \frac{b_1}{1^{-2}}
+ \frac{b_2}{2^{-2}} \right) \\
%
h_{(2,-4)} &=
  \elf_3(1) \left(
  \frac{b_1}{1^{-4}}
+ \frac{b_2}{2^{-4}} \right) \\
%
&\ldots \\
%
j_{(2,0)} &=
- \elg_{-1}(1) \left(
  \frac{b_1}{1^0}
+ \frac{b_2}{2^0} \right)
+ \xi_0 \\
%
j_{(2,2)} &=
- \elg_{-3}(1) \left(
  \frac{b_1}{1^2}
+ \frac{b_2}{2^2} \right)
+ \xi_2 \\
%
&\ldots \\
\end{aligned} \right. \end{equation*}
%
\begin{equation*} \left| \begin{aligned}
%
h_{(3,-2)} &=
  \elf_1(1) \left(
  \frac{b_1}{1^{-2}}
+ \frac{b_2}{2^{-2}}
+ \frac{b_3}{3^{-2}} \right) \\
%
h_{(3,-4)} &=
  \elf_3(1) \left(
  \frac{b_1}{1^{-4}}
+ \frac{b_2}{2^{-4}}
+ \frac{b_3}{3^{-4}} \right) \\
%
&\ldots \\
%
j_{(3,0)} &=
- \elg_{-1}(1) \left(
  \frac{b_1}{1^0}
+ \frac{b_2}{2^0}
+ \frac{b_3}{3^0} \right)
+ \xi_0 \\
%
j_{(3,2)} &=
- \elg_{-3}(1) \left(
  \frac{b_1}{1^2}
+ \frac{b_2}{2^2}
+ \frac{b_3}{3^2} \right)
+ \xi_2 \\
%
&\ldots \\
\end{aligned} \right. \end{equation*}
%
\begin{equation*} \left| \begin{aligned}
h_{(n,-2)} &=
  \elf_1(1) \left(
  \frac{b_1}{1^{-2}}
+ \frac{b_2}{2^{-2}}
+ \frac{b_3}{3^{-2}}
+ \ldots
+ \frac{b_n}{n^{-2}} \right) \\
%
h_{(n,-4)} &=
  \elf_3(1) \left(
  \frac{b_1}{1^{-4}}
+ \frac{b_2}{2^{-4}}
+ \frac{b_3}{3^{-4}}
+ \ldots
+ \frac{b_n}{n^{-4}} \right) \\
%
&\ldots \\
%
j_{(n,0)} &=
- \elg_{-1}(1) \left(
  \frac{b_1}{1^0}
+ \frac{b_2}{2^0}
+ \frac{b_3}{3^0}
+ \ldots
+ \frac{b_n}{n^0} \right)
+ \xi_0 \\
%
j_{(n,2)} &=
- \elg_{-3}(1) \left(
  \frac{b_1}{1^2}
+ \frac{b_2}{2^2}
+ \frac{b_3}{3^2}
+ \ldots
+ \frac{b_n}{n^2} \right)
+ \xi_2 \\
%
&\ldots \\
\end{aligned} \right. \end{equation*}