% !TeX root = sincotsec.tex

\subsection{Натуральные корни}

\begin{equation*} \begin{aligned}
&A(x) =
  \frac{\theta_1}{1 + \cfrac{x}{1}}
+ \frac{\theta_2}{1 + \cfrac{x}{2}}
+ \frac{\theta_3}{1 + \cfrac{x}{3}}
+ \ldots
+ \frac{\theta_n}{1 + \cfrac{x}{n}}
\end{aligned} \end{equation*}

\begin{equation*} \begin{aligned}
\theta_1 &= \frac{1}{
  \left(1 - \displaystyle \frac{1}{2} \right)
  \left(1 - \displaystyle \frac{1}{3} \right)
  \cdot \ldots \cdot
  \left(1 - \displaystyle \frac{1}{{n - 1}} \right)
  \left(1 - \displaystyle \frac{1}{n} \right)} \\
\theta_2 &= \frac{1}{
  \left(1 - \displaystyle \frac{2}{1} \right)
  \left(1 - \displaystyle \frac{2}{3} \right)
  \cdot \ldots \cdot
  \left(1 - \displaystyle \frac{2}{{n - 1}} \right)
  \left(1 - \displaystyle \frac{2}{n} \right)} \\
\theta_3 &= \frac{1}{
  \left(1 - \displaystyle \frac{3}{1} \right)
  \left(1 - \displaystyle \frac{3}{2} \right)
  \cdot \ldots \cdot
  \left(1 - \displaystyle \frac{3}{{n - 1}} \right)
  \left(1 - \displaystyle \frac{3}{n} \right)} \\
&\ldots \\
\theta_n &= \frac{1}{
  \left(1 - \displaystyle \frac{n}{1} \right)
  \left(1 - \displaystyle \frac{n}{2} \right)
  \left(1 - \displaystyle \frac{n}{3} \right)
  \cdot \ldots \cdot
  \left(1 - \displaystyle \frac{n}{{n - 1}} \right)} \\
\end{aligned} \end{equation*}

\begin{equation*} \begin{aligned}
\theta_1 &=
  \displaystyle \frac{n}{1} \\
\theta_2 &=
  \displaystyle \frac{n}{2}
  \displaystyle \frac{n - 1}{-1} \\
\theta_3 &=
  \displaystyle \frac{n}{3}
  \displaystyle \frac{n - 1}{-1}
  \displaystyle \frac{n - 2}{-2} \\
&\ldots \\
\theta_n &=
  \displaystyle \frac{n}{n}
  \displaystyle \frac{n - 1}{-1}
  \displaystyle \frac{n - 2}{-2}
  \displaystyle \frac{n - 3}{-3}
  \cdot \ldots \cdot
  \displaystyle \frac{1}{-(n - 1)}
  \\
\end{aligned} \end{equation*}

\begin{equation*} \begin{aligned}
\theta_1 &=
  \displaystyle \frac{n!}{1!(n - 1)!} \\
\theta_2 &=
  - \displaystyle \frac{n!}{2!(n - 2)!} \\
\theta_3 &=
  \displaystyle \frac{n!}{3!(n - 3)!} \\
&\ldots \\
\theta_n &=
  -(-1)^n \displaystyle \frac{n!}{n!0!} \\
  \\
\end{aligned} \end{equation*}

\begin{equation*} \left| \begin{aligned}
A(x) &= \Psi(x) & 
&|x| < 1 \\
%
A(x) &= S_1(x) & 
1 < &|x| < 2 \\
%
A(x) &= S_2(x) & 
2 < &|x| < 3 \\
%
A(x) &= S_3(x) &
3 < &|x| < 4 \\
&\ldots & & \\
%
A(x) &= S_n(x) &
n < &|x| \\
\end{aligned} \right. \end{equation*}

\begin{equation*} \left| \begin{aligned}
\Psi(x) &=
  \psi_0 \elf_0(x)
+ \psi_1 \elf_1(x) 
+ \psi_2 \elf_2(x) 
+ \psi_3 \elf_3(x) 
+ \ldots \\
%
S_1(x) &= 
  s_{(1,-1)} \elg_{-1}(x)
+ s_{(1,-2)} \elg_{-2}(x)
+ s_{(1,-3)} \elg_{-3}(x)
+ s_{(1,-4)} \elg_{-4}(x)
+ \ldots \\ &
+ t_{(1,0)} \elf_0(x)
+ t_{(1,1)} \elf_1(x)
+ t_{(1,2)} \elf_2(x)
+ t_{(1,3)} \elf_3(x)
+ \ldots \\
%
S_2(x) &= 
  s_{(2,-1)} \elg_{-1}(x)
+ s_{(2,-2)} \elg_{-2}(x)
+ s_{(2,-3)} \elg_{-3}(x)
+ s_{(2,-4)} \elg_{-4}(x)
+ \ldots \\ &
+ t_{(2,0)} \elf_0(x)
+ t_{(2,1)} \elf_1(x)
+ t_{(2,2)} \elf_2(x)
+ t_{(2,3)} \elf_3(x)
+ \ldots \\
%
S_3(x) &= 
  s_{(3,-1)} \elg_{-1}(x)
+ s_{(3,-2)} \elg_{-2}(x)
+ s_{(3,-3)} \elg_{-3}(x)
+ s_{(3,-4)} \elg_{-4}(x)
+ \ldots \\ &
+ t_{(3,0)} \elf_0(x)
+ t_{(3,1)} \elf_1(x)
+ t_{(3,2)} \elf_2(x)
+ t_{(3,3)} \elf_3(x)
+ \ldots \\
%
&\ldots \\
%
S_n(x) &= 
  s_{(n,-1)} \elg_{-1}(x)
+ s_{(n,-2)} \elg_{-2}(x)
+ s_{(n,-3)} \elg_{-3}(x)
+ s_{(n,-4)} \elg_{-4}(x)
+ \ldots \\ &
+ t_{(n,0)} \elf_0(x)
+ t_{(n,1)} \elf_1(x)
+ t_{(n,2)} \elf_2(x)
+ t_{(n,3)} \elf_3(x)
+ \ldots \\
\end{aligned} \right. \end{equation*}

\begin{equation*} \left| \begin{aligned}
\psi_0 &= \elg_{-1}(1) \left(
  \frac{\theta_1}{1^0}
+ \frac{\theta_2}{2^0}
+ \frac{\theta_3}{3^0}
+ \ldots
+ \frac{\theta_n}{n^0} \right) \\
%
\psi_1 &= \elg_{-2}(1) \left(
  \frac{\theta_1}{1^1}
+ \frac{\theta_2}{2^1}
+ \frac{\theta_3}{3^1}
+ \ldots
+ \frac{\theta_n}{n^1} \right) \\
%
\psi_2 &= \elg_{-3}(1) \left(
  \frac{\theta_1}{1^2}
+ \frac{\theta_2}{2^2}
+ \frac{\theta_3}{3^2}
+ \ldots
+ \frac{\theta_n}{n^2} \right) \\
%
\psi_3 &= \elg_{-4}(1) \left(
  \frac{\theta_1}{1^3}
+ \frac{\theta_2}{2^3}
+ \frac{\theta_3}{3^3}
+ \ldots
+ \frac{\theta_n}{n^3} \right) \\
%
&\ldots \\
\end{aligned} \right. \end{equation*}

\begin{equation*} \left| \begin{aligned}
%
s_{(1,-1)} &=
  \elf_0(1) \frac{\theta_1}{1^{-1}} \\
%
s_{(1,-2)} &=
  \elf_1(1) \frac{\theta_1}{1^{-2}} \\
%
s_{(1,-3)} &=
  \elf_2(1) \frac{\theta_1}{1^{-3}} \\
%
s_{(1,-4)} &=
  \elf_3(1) \frac{\theta_1}{1^{-4}} \\
%
&\ldots \\
%
t_{(1,0)} &=
- \elg_{-1}(1) \frac{\theta_1}{1^0}
+ \psi_0 \\
%
t_{(1,1)} &=
- \elg_{-2}(1) \frac{\theta_1}{1^1}
+ \psi_1 \\
%
t_{(1,2)} &=
- \elg_{-3}(1) \frac{\theta_1}{1^2}
+ \psi_2 \\
%
t_{(1,3)} &=
- \elg_{-4}(1) \frac{\theta_1}{1^3}
+ \psi_3 \\
%
&\ldots \\
\end{aligned} \right. \end{equation*}

\begin{equation*} \left| \begin{aligned}
s_{(2,-1)} &=
  \elf_0(1) \left(
  \frac{\theta_1}{1^{-1}}
+ \frac{\theta_2}{2^{-1}} \right) \\
%
s_{(2,-2)} &=
  \elf_1(1) \left(
  \frac{\theta_1}{1^{-2}}
+ \frac{\theta_2}{2^{-2}} \right) \\
%
s_{(2,-3)} &=
  \elf_2(1) \left(
  \frac{\theta_1}{1^{-3}}
+ \frac{\theta_2}{2^{-3}} \right) \\
%
s_{(2,-4)} &=
  \elf_3(1) \left(
  \frac{\theta_1}{1^{-4}}
+ \frac{\theta_2}{2^{-4}} \right) \\
%
&\ldots \\
%
t_{(2,0)} &=
- \elg_{-1}(1) \left(
  \frac{\theta_1}{1^0}
+ \frac{\theta_2}{2^0} \right)
+ \psi_0 \\
%
t_{(2,1)} &=
- \elg_{-2}(1) \left(
  \frac{\theta_1}{1^1}
+ \frac{\theta_2}{2^1} \right)
+ \psi_1 \\
%
t_{(2,2)} &=
- \elg_{-3}(1) \left(
  \frac{\theta_1}{1^2}
+ \frac{\theta_2}{2^2} \right)
+ \psi_2 \\
%
t_{(2,3)} &=
- \elg_{-4}(1) \left(
  \frac{\theta_1}{1^3}
+ \frac{\theta_2}{2^3} \right)
+ \psi_3 \\
%
&\ldots \\
\end{aligned} \right. \end{equation*}
%
\begin{equation*} \left| \begin{aligned}
%
s_{(3,-1)} &=
  \elf_0(1) \left(
  \frac{\theta_1}{1^{-1}}
+ \frac{\theta_2}{2^{-1}}
+ \frac{\theta_3}{3^{-1}} \right) \\
%
s_{(3,-2)} &=
  \elf_1(1) \left(
  \frac{\theta_1}{1^{-2}}
+ \frac{\theta_2}{2^{-2}}
+ \frac{\theta_3}{3^{-2}} \right) \\
%
s_{(3,-3)} &=
  \elf_2(1) \left(
  \frac{\theta_1}{1^{-3}}
+ \frac{\theta_2}{2^{-3}}
+ \frac{\theta_3}{3^{-3}} \right) \\
%
s_{(3,-4)} &=
  \elf_3(1) \left(
  \frac{\theta_1}{1^{-4}}
+ \frac{\theta_2}{2^{-4}}
+ \frac{\theta_3}{3^{-4}} \right) \\
%
&\ldots \\
%
t_{(3,0)} &=
- \elg_{-1}(1) \left(
  \frac{\theta_1}{1^0}
+ \frac{\theta_2}{2^0}
+ \frac{\theta_3}{3^0} \right)
+ \psi_0 \\
%
t_{(3,1)} &=
- \elg_{-2}(1) \left(
  \frac{\theta_1}{1^1}
+ \frac{\theta_2}{2^1}
+ \frac{\theta_3}{3^1} \right)
+ \psi_1 \\
%
t_{(3,2)} &=
- \elg_{-3}(1) \left(
  \frac{\theta_1}{1^2}
+ \frac{\theta_2}{2^2}
+ \frac{\theta_3}{3^2} \right)
+ \psi_2 \\
%
t_{(3,3)} &=
- \elg_{-4}(1) \left(
  \frac{\theta_1}{1^3}
+ \frac{\theta_2}{2^3}
+ \frac{\theta_3}{3^3} \right)
+ \psi_3 \\
%
&\ldots \\
\end{aligned} \right. \end{equation*}
%
\begin{equation*} \left| \begin{aligned}
s_{(n,-1)} &=
  \elf_0(1) \left(
  \frac{\theta_1}{1^{-1}}
+ \frac{\theta_2}{2^{-1}}
+ \frac{\theta_3}{3^{-1}}
+ \ldots
+ \frac{\theta_n}{n^{-1}} \right) \\
%
s_{(n,-2)} &=
  \elf_1(1) \left(
  \frac{\theta_1}{1^{-2}}
+ \frac{\theta_2}{2^{-2}}
+ \frac{\theta_3}{3^{-2}}
+ \ldots
+ \frac{\theta_n}{n^{-2}} \right) \\
%
s_{(n,-3)} &=
  \elf_2(1) \left(
  \frac{\theta_1}{1^{-3}}
+ \frac{\theta_2}{2^{-3}}
+ \frac{\theta_3}{3^{-3}}
+ \ldots
+ \frac{\theta_n}{n^{-3}} \right) \\
%
s_{(n,-4)} &=
  \elf_3(1) \left(
  \frac{\theta_1}{1^{-4}}
+ \frac{\theta_2}{2^{-4}}
+ \frac{\theta_3}{3^{-4}}
+ \ldots
+ \frac{\theta_n}{n^{-4}} \right) \\
%
&\ldots \\
%
t_{(n,0)} &=
- \elg_{-1}(1) \left(
  \frac{\theta_1}{1^0}
+ \frac{\theta_2}{2^0}
+ \frac{\theta_3}{3^0}
+ \ldots
+ \frac{\theta_n}{n^0} \right)
+ \psi_0 \\
%
t_{(n,1)} &=
- \elg_{-2}(1) \left(
  \frac{\theta_1}{1^1}
+ \frac{\theta_2}{2^1}
+ \frac{\theta_3}{3^1}
+ \ldots
+ \frac{\theta_n}{n^1} \right)
+ \psi_1 \\
%
t_{(n,2)} &=
- \elg_{-3}(1) \left(
  \frac{\theta_1}{1^2}
+ \frac{\theta_2}{2^2}
+ \frac{\theta_3}{3^2}
+ \ldots
+ \frac{\theta_n}{n^2} \right)
+ \psi_2 \\
%
t_{(n,3)} &=
- \elg_{-4}(1) \left(
  \frac{\theta_1}{1^3}
+ \frac{\theta_2}{2^3}
+ \frac{\theta_3}{3^3}
+ \ldots
+ \frac{\theta_n}{n^3} \right)
+ \psi_3 \\
%
&\ldots \\
\end{aligned} \right. \end{equation*}