% !TeX root = sincotsec.tex

\subsection{Симметричные натуральные корни}

\begin{equation*} \begin{aligned}
B(x) &=
  \ln{\left(1 + \frac{x}{1} \right)}
+ \ln{\left(1 + \frac{x}{2} \right)}
+ \ln{\left(1 + \frac{x}{3} \right)}
+ \ldots
+ \ln{\left(1 + \frac{x}{n} \right)} \\ &
+ \ln{\left(1 - \frac{x}{1} \right)}
+ \ln{\left(1 - \frac{x}{2} \right)}
+ \ln{\left(1 - \frac{x}{3} \right)}
+ \ldots
+ \ln{\left(1 - \frac{x}{n} \right)}
\end{aligned} \end{equation*}

\begin{equation*} \left| \begin{aligned}
B(x) &= \Xi(x) & 
&|x| < 1 \\
%
B(x) &= G_1(x) & 
1 < &|x| < 2 \\
%
B(x) &= G_2(x) & 
2 < &|x| < 3 \\
%
B(x) &= G_3(x) &
3 < &|x| < 4 \\
&\ldots & & \\
%
B(x) &= G_n(x) &
n < &|x| \\
\end{aligned} \right. \end{equation*}

\begin{equation*} \left| \begin{aligned}
\Xi(x) &=
  \xi_0 \elf_0(x)
+ \xi_2 \elf_2(x) 
+ \ldots \\
%
G_1(x) &=
  g_{(1,0)} \elg_0(x) 
+ g_{(1,-2)} \elg_{-2}(x)
+ \ldots \\ &
+ h_{(1,0)} \elf_0(x)
+ h_{(1,2)} \elf_2(x)
+ \ldots \\
%
G_2(x) &=
  g_{(2,0)} \elg_0(x) 
+ g_{(2,-2)} \elg_{-2}(x)
+ \ldots \\ &
+ h_{(2,0)} \elf_0(x)
+ h_{(2,2)} \elf_2(x)
+ \ldots \\
%
G_3(x) &=
  g_{(3,0)} \elg_0(x) 
+ g_{(3,-2)} \elg_{-2}(x)
+ \ldots \\ &
+ h_{(3,0)} \elf_0(x)
+ h_{(3,2)} \elf_2(x)
+ \ldots \\
%
&\ldots \\
%
G_n(x) &=
  g_{(n,0)} \elg_0(x) 
+ g_{(n,-2)} \elg_{-2}(x)
+ \ldots \\ &
+ h_{(n,0)} \elf_0(x)
+ h_{(n,2)} \elf_2(x)
+ \ldots \\
\end{aligned} \right. \end{equation*}

\begin{equation*} \left| \begin{aligned}
\xi_0 &= 2 \elg_0(1) \left(
  \frac{1}{1^0}
+ \frac{1}{2^0}
+ \frac{1}{3^0}
+ \ldots
+ \frac{1}{n^0} \right) \\
%
\xi_2 &= 2 \elg_{-2}(1) \left(
  \frac{1}{1^2}
+ \frac{1}{2^2}
+ \frac{1}{3^2}
+ \ldots
+ \frac{1}{n^2} \right) \\
%
\xi_4 &= 2 \elg_{-4}(1) \left(
  \frac{1}{1^4}
+ \frac{1}{2^4}
+ \frac{1}{3^4}
+ \ldots
+ \frac{1}{n^4} \right) \\
%
&\ldots \\
\end{aligned} \right. \end{equation*}

\begin{equation*} \left| \begin{aligned}
g_{(1,0)} &=
  2 \elf_0(1) \frac{1}{1^0} \\
%
g_{(1,-2)} &=
  2 \elf_2(1) \frac{1}{1^{-2}} \\
%
g_{(1,-4)} &=
  2 \elf_4(1) \frac{1}{1^{-4}} \\
%
&\ldots \\
%
h_{(1,0)} &=
- 2 \elg_0(1) \frac{1}{1^0}
- \elf_0(1) \frac{\ln{(-1^2)}}{1^0}
+ \xi_0 \\
%
h_{(1,2)} &=
- 2 \elg_{-2}(1) \frac{1}{1^2}
+ \xi_2 \\
%
&\ldots \\
\end{aligned} \right. \end{equation*}

\begin{equation*} \left| \begin{aligned}
g_{(2,0)} &=
  2 \elf_0(1) \left(
  \frac{1}{1^0}
+ \frac{1}{2^0} \right) \\
%
g_{(2,-2)} &=
  2 \elf_2(1) \left(
  \frac{1}{1^{-2}}
+ \frac{1}{2^{-2}} \right) \\
%
g_{(2,-4)} &=
  2 \elf_4(1) \left(
  \frac{1}{1^{-4}}
+ \frac{1}{2^{-4}} \right) \\
%
&\ldots \\
%
h_{(2,0)} &=
- 2 \elg_0(1) \left(
  \frac{1}{1^0}
+ \frac{1}{2^0} \right)
- \elf_0(1) \left(
  \frac{\ln{(-1^2)}}{1^0}
+ \frac{\ln{(-2^2)}}{2^0} \right)
+ \xi_0 \\
%
h_{(2,2)} &=
- 2 \elg_{-2}(1) \left(
  \frac{1}{1^2}
+ \frac{1}{2^2} \right)
+ \xi_2 \\
%
&\ldots \\
\end{aligned} \right. \end{equation*}

\begin{equation*} \left| \begin{aligned}
g_{(3,0)} &=
  2 \elf_0(1) \left(
  \frac{1}{1^0}
+ \frac{1}{2^0}
+ \frac{1}{3^0} \right) \\
%
g_{(3,-2)} &=
  2 \elf_2(1) \left(
  \frac{1}{1^{-2}}
+ \frac{1}{2^{-2}}
+ \frac{1}{3^{-2}} \right) \\
%
g_{(3,-4)} &=
  2 \elf_4(1) \left(
  \frac{1}{1^{-4}}
+ \frac{1}{2^{-4}}
+ \frac{1}{3^{-4}} \right) \\
%
&\ldots \\
%
h_{(3,0)} &=
- 2 \elg_0(1) \left(
  \frac{1}{1^0}
+ \frac{1}{2^0}
+ \frac{1}{3^0} \right)
- \elf_0(1) \left(
  \frac{\ln{(-1^2)}}{1^0}
+ \frac{\ln{(-2^2)}}{2^0}
+ \frac{\ln{(-3^2)}}{3^0} \right)
+ \xi_0 \\
%
h_{(3,2)} &=
- 2 \elg_{-2}(1) \left(
  \frac{1}{1^2}
+ \frac{1}{2^2}
+ \frac{1}{3^2} \right)
+ \xi_2 \\
%
&\ldots \\
\end{aligned} \right. \end{equation*}
%
\begin{equation*} \left| \begin{aligned}
g_{(n,0)} &=
  2 \elf_0(1) \left(
  \frac{1}{1^0}
+ \frac{1}{2^0}
+ \frac{1}{3^0}
+ \ldots
+ \frac{1}{n^0} \right) \\
%
g_{(n,-2)} &=
  2 \elf_2(1) \left(
  \frac{1}{1^{-2}}
+ \frac{1}{2^{-2}}
+ \frac{1}{3^{-2}}
+ \ldots
+ \frac{1}{n^{-2}} \right) \\
%
g_{(n,-4)} &=
  2 \elf_4(1) \left(
  \frac{1}{1^{-4}}
+ \frac{1}{2^{-4}}
+ \frac{1}{3^{-4}}
+ \ldots
+ \frac{1}{n^{-4}} \right) \\
%
&\ldots \\
%
h_{(n,0)} &=
- 2 \elg_0(1) \left(
  \frac{1}{1^0}
+ \frac{1}{2^0}
+ \frac{1}{3^0}
+ \ldots
+ \frac{1}{n^0} \right) \\ &
- \elf_0(1) \left(
  \frac{\ln{(-1^2)}}{1^0}
+ \frac{\ln{(-2^2)}}{2^0}
+ \frac{\ln{(-3^2)}}{3^0}
+ \ldots
+ \frac{\ln{(-n^2)}}{n^0} \right)
+ \xi_0 \\
%
h_{(n,2)} &=
- 2 \elg_{-2}(1) \left(
  \frac{1}{1^2}
+ \frac{1}{2^2}
+ \frac{1}{3^2}
+ \ldots
+ \frac{1}{n^2} \right)
+ \xi_2 \\
%
&\ldots \\
\end{aligned} \right. \end{equation*}