% !TeX root = sincotsec.tex

\section{$\omega_0$-функции}

\begin{equation*}\begin{aligned}
&\ldots \\
\omega_{(0,0)}(x) &= \frac{x^0}{0!} \\
\omega_{(0,1)}(x) &= \frac{x^1}{1!} \\
\omega_{(0,2)}(x) &= \frac{x^2}{2!} \\
\omega_{(0,3)}(x) &= \frac{x^3}{3!} \\
\omega_{(0,4)}(x) &= \frac{x^4}{4!} \\
&\ldots \\
\end{aligned}\end{equation*}

\begin{equation*}
\lim_{p \to 0} \frac{\omega_{(0, n)}(x + p) - \omega_{(0, n)}(x)}{p} = \omega_{(0, n - 1)}(x) \\
\end{equation*}

\begin{equation*} \begin{aligned}
\omega_{(0,0)}(x_1 + x_2) &=  
  \omega_0(x_1) \omega_0(x_2) \\
%
\omega_{(0,1)}(x_1 + x_2) &=  
  \omega_1(x_1) \omega_0(x_2)
+ \omega_0(x_1) \omega_1(x_2) \\
%
\omega_{(0,2)}(x_1 + x_2) &=  
  \omega_2(x_1) \omega_0(x_2)
+ \omega_1(x_1) \omega_1(x_2)
+ \omega_0(x_1) \omega_2(x_2) \\
%
\omega_{(0,3)}(x_1 + x_2) &=  
  \omega_3(x_1) \omega_0(x_2)
+ \omega_2(x_1) \omega_1(x_2)
+ \omega_1(x_1) \omega_2(x_2)
+ \omega_0(x_1) \omega_3(x_2) \\
%
\omega_{(0,4)}(x_1 + x_2) &=  
  \omega_4(x_1) \omega_0(x_2)
+ \omega_3(x_1) \omega_1(x_2)
+ \omega_2(x_1) \omega_2(x_2)
+ \omega_1(x_1) \omega_3(x_2)
+ \omega_0(x_1) \omega_4(x_2) \\
%
&\ldots \\
\end{aligned} \end{equation*}

\begin{equation*} \begin{aligned}
\omega_{(0,0)}(x_1 + x_2 + x_3) &=  
  \omega_0(x_1) \omega_0(x_2) \omega_0(x_3) \\
%
\omega_{(0,1)}(x_1 + x_2 + x_3) &=  
  \omega_1(x_1) \omega_0(x_2) \omega_0(x_3)
+ \omega_0(x_1) \omega_1(x_2) \omega_0(x_3)
+ \omega_0(x_1) \omega_0(x_2) \omega_1(x_3) \\
%
\omega_{(0,2)}(x_1 + x_2 + x_3) &=  
  \omega_2(x_1) \omega_0(x_2) \omega_0(x_3)
+ \omega_1(x_1) \omega_1(x_2) \omega_0(x_3)
+ \omega_1(x_1) \omega_0(x_2) \omega_1(x_3) \\ &
+ \omega_0(x_1) \omega_2(x_2) \omega_0(x_3)
+ \omega_0(x_1) \omega_1(x_2) \omega_1(x_3)
+ \omega_0(x_1) \omega_0(x_2) \omega_2(x_3) \\
%
\omega_{(0,3)}(x_1 + x_2 + x_3) &=  
  \omega_3(x_1) \omega_0(x_2) \omega_0(x_3)
+ \omega_2(x_1) \omega_1(x_2) \omega_0(x_3)
+ \omega_2(x_1) \omega_0(x_2) \omega_1(x_3) \\ &
+ \omega_1(x_1) \omega_2(x_2) \omega_0(x_3)
+ \omega_1(x_1) \omega_1(x_2) \omega_1(x_3)
+ \omega_1(x_1) \omega_0(x_2) \omega_2(x_3) \\ &
+ \omega_0(x_1) \omega_3(x_2) \omega_0(x_3)
+ \omega_0(x_1) \omega_2(x_2) \omega_1(x_3)
+ \omega_0(x_1) \omega_1(x_2) \omega_2(x_3) \\ &
+ \omega_0(x_1) \omega_0(x_2) \omega_3(x_3) \\
%
\omega_{(0,4)}(x_1 + x_2 + x_3) &=  
  \omega_4(x_1) \omega_0(x_2) \omega_0(x_3)
+ \omega_3(x_1) \omega_1(x_2) \omega_0(x_3)
+ \omega_3(x_1) \omega_0(x_2) \omega_1(x_3) \\ &
+ \omega_2(x_1) \omega_2(x_2) \omega_0(x_3)
+ \omega_2(x_1) \omega_1(x_2) \omega_1(x_3)
+ \omega_2(x_1) \omega_0(x_2) \omega_2(x_3) \\ &
+ \omega_1(x_1) \omega_3(x_2) \omega_0(x_3)
+ \omega_1(x_1) \omega_2(x_2) \omega_1(x_3)
+ \omega_1(x_1) \omega_1(x_2) \omega_2(x_3) \\ &
+ \omega_1(x_1) \omega_0(x_2) \omega_3(x_3)
+ \omega_0(x_1) \omega_4(x_2) \omega_0(x_3)
+ \omega_0(x_1) \omega_3(x_2) \omega_1(x_3) \\ &
+ \omega_0(x_1) \omega_2(x_2) \omega_2(x_3)
+ \omega_0(x_1) \omega_1(x_2) \omega_3(x_3)
+ \omega_0(x_1) \omega_0(x_2) \omega_4(x_3) \\
%
&\ldots \\
\end{aligned} \end{equation*}

\begin{equation*}
\begin{aligned}
\frac{(1 + x)^0}{0!} &=
  \frac{1}{0!0!} 
\\
\frac{(1 + x)^1}{1!} &=
  \frac{1}{1!0!} 
+ \frac{1}{0!1!} x
\\
\frac{(1 + x)^2}{2!} &= 
  \frac{1}{2!0!} 
+ \frac{1}{1!1!} x 
+ \frac{1}{0!2!} x^2
\\
\frac{(1 + x)^3}{3!} &=
  \frac{1}{3!0!} 
+ \frac{1}{2!1!} x 
+ \frac{1}{1!2!} x^2 
+ \frac{1}{0!3!} x^3
\\
\frac{(1 + x)^4}{4!} &=
  \frac{1}{4!0!} 
+ \frac{1}{3!1!} x 
+ \frac{1}{2!2!} x^2 
+ \frac{1}{1!3!} x^3 
+ \frac{1}{0!4!} x^4
\\
\frac{(1 + x)^5}{5!} &=
  \frac{1}{5!0!} 
+ \frac{1}{4!1!} x 
+ \frac{1}{3!2!} x^2 
+ \frac{1}{2!3!} x^3 
+ \frac{1}{1!4!} x^4
+ \frac{1}{0!5!} x^5
\\
&\ldots
\\
\end{aligned}
\end{equation*}

\begin{equation*}
\begin{aligned}
(1 + x)^1 &=
  \frac{1!}{1!0!} 
+ \frac{1!}{0!1!} x
\\
(1 + x)^2 &= 
  \frac{2!}{2!0!} 
+ \frac{2!}{1!1!} x 
+ \frac{2!}{0!2!} x^2
\\
(1 + x)^3 &=
  \frac{3!}{3!0!} 
+ \frac{3!}{2!1!} x 
+ \frac{3!}{1!2!} x^2 
+ \frac{3!}{0!3!} x^3
\\
(1 + x)^4 &=
  \frac{4!}{4!0!} 
+ \frac{4!}{3!1!} x 
+ \frac{4!}{2!2!} x^2 
+ \frac{4!}{1!3!} x^3 
+ \frac{4!}{0!4!} x^4
\\
(1 + x)^5 &=
  \frac{5!}{5!0!} 
+ \frac{5!}{4!1!} x 
+ \frac{5!}{3!2!} x^2 
+ \frac{5!}{2!3!} x^3 
+ \frac{5!}{1!4!} x^4
+ \frac{5!}{0!5!} x^5
\\
&\ldots
\\
\end{aligned}
\end{equation*}

\begin{equation*}
C(x) = c_0 + c_1 x + c_2 x^2 + c_3 x^3 + c_4 x^4 + \ldots \\
\end{equation*}

\begin{equation*} \begin{aligned}
\omega_{(0,0)}(C) &= h_{(0,0)} + h_{(0,1)} x + h_{(0,2)} x^2 + h_{(0,3)} x^3 + \ldots \\
\omega_{(0,1)}(C) &= h_{(1,0)} + h_{(1,1)} x + h_{(1,2)} x^2 + h_{(1,3)} x^3 + \ldots \\
\omega_{(0,2)}(C) &= h_{(2,0)} + h_{(2,1)} x + h_{(2,2)} x^2 + h_{(2,3)} x^3 + \ldots \\
\omega_{(0,3)}(C) &= h_{(3,0)} + h_{(3,1)} x + h_{(3,2)} x^2 + h_{(3,3)} x^3 + \ldots \\
\omega_{(0,4)}(C) &= h_{(4,0)} + h_{(4,1)} x + h_{(4,2)} x^2 + h_{(4,3)} x^3 + \ldots \\
\omega_{(0,5)}(C) &= h_{(5,0)} + h_{(5,1)} x + h_{(5,2)} x^2 + h_{(5,3)} x^3 + \ldots \\
&\ldots \\
\end{aligned} \end{equation*}

\begin{equation*} \left| \begin{aligned} 
h_{(0,0)} &= 1 \\ 
h_{(0,1)} &= 0 \\
h_{(0,2)} &= 0 \\
h_{(0,3)} &= 0 \\
h_{(0,4)} &= 0 \\
h_{(0,5)} &= 0 \\
h_{(0,6)} &= 0 \\
&\ldots
\end{aligned} \right. \end{equation*}

\begin{equation*} \left| \begin{aligned} 
h_{(1,0)} &= \frac{c_0}{1!} \\ 
h_{(1,1)} &= \frac{c_1}{1!} \\
h_{(1,2)} &= \frac{c_2}{1!} \\
h_{(1,3)} &= \frac{c_3}{1!} \\
h_{(1,4)} &= \frac{c_4}{1!} \\
h_{(1,5)} &= \frac{c_5}{1!} \\
h_{(1,6)} &= \frac{c_6}{1!} \\
&\ldots
\end{aligned} \right. \end{equation*}

\begin{equation*} \left| \begin{aligned} 
h_{(2,0)} &=
  \frac{c_0^2}{2!} \\
%
h_{(2,1)} &=
  \frac{c_1 c_0}{1!1!} \\
%
h_{(2,2)} &=
  \frac{c_2 c_0}{1!1!}
+ \frac{c_1^2}{2!} \\
%
h_{(2,3)} &=
  \frac{c_3 c_0}{1!1!}
+ \frac{c_2 c_1}{1!1!} \\
%
h_{(2,4)} &=
  \frac{c_4 c_0}{1!1!}
+ \frac{c_3 c_1}{1!1!}
+ \frac{c_2^2}{2!} \\
%
h_{(2,5)} &=
  \frac{c_5 c_0}{1!1!}
+ \frac{c_4 c_1}{1!1!}
+ \frac{c_3 c_2}{1!1!} \\
%
h_{(2,6)} &=
  \frac{c_6 c_0}{1!1!}
+ \frac{c_5 c_1}{1!1!}
+ \frac{c_4 c_2}{1!1!}
+ \frac{c_3^2}{2!} \\
%
&\ldots
\end{aligned} \right. \end{equation*}

\begin{equation*} \left| \begin{aligned}
h_{(3,0)} &=
  \frac{c_0^3}{3!} \\ 
%
h_{(3,1)} &=
  \frac{c_1 c_0^2}{1!2!} \\
%
h_{(3,2)} &=
  \frac{c_2 c_0^2}{1!2!} 
+ \frac{c_1^2 c_0}{2!1!} \\
%
h_{(3,3)} &=
  \frac{c_3 c_0^2}{1!2!} 
+ \frac{c_2 c_1 c_0}{1!1!1!} 
+ \frac{c_1^3}{3!} \\
%
h_{(3,4)} &=
  \frac{c_4 c_0^2}{1!2!} 
+ \frac{c_3 c_1 c_0}{1!1!1!} 
+ \frac{c_2^2 c_0}{2!1!} 
+ \frac{c_2 c_1^2}{1!2!} \\
%
h_{(3,5)} &=
  \frac{c_5 c_0^2}{1!2!} 
+ \frac{c_4 c_1 c_0}{1!1!1!} 
+ \frac{c_3 c_2 c_0}{1!1!1!} 
+ \frac{c_3 c_1^2}{1!2!}
+ \frac{c_2^2 c_1}{2!1!} \\
%
h_{(3,6)} &=
  \frac{c_6 c_0^2}{1!2!} 
+ \frac{c_5 c_1 c_0}{1!1!1!} 
+ \frac{c_4 c_2 c_0}{1!1!1!} 
+ \frac{c_4 c_1^2}{1!2!}
+ \frac{c_3^2 c_0}{2!1!} 
+ \frac{c_3 c_2 c_1}{1!1!1!} 
+ \frac{c_2^3}{3!} \\
%
&\ldots
\end{aligned} \right. \end{equation*}

\begin{equation*} \left| \begin{aligned} 
h_{(4,0)} &=
  \frac{c_0^4}{4!} \\ 
%
h_{(4,1)} &=
  \frac{c_1 c_0^3}{1!3!} \\
%
h_{(4,2)} &=
  \frac{c_2 c_0^3}{1!3!} 
+ \frac{c_1^2 c_0^2}{2!2!} \\
%
h_{(4,3)} &=
  \frac{c_3 c_0^3}{1!3!} 
+ \frac{c_2 c_1 c_0^2}{1!1!2!} 
+ \frac{c_1^3 c_0}{3!1!} \\
%
h_{(4,4)} &=
  \frac{c_4 c_0^3}{1!3!} 
+ \frac{c_3 c_1 c_0^2}{1!1!2!} 
+ \frac{c_2^2 c_0^2}{2!2!}
+ \frac{c_2 c_1^2 c_0}{1!2!1!} 
+ \frac{c_1^4}{4!} \\
%
h_{(4,5)} &=
  \frac{c_5 c_0^3}{1!3!} 
+ \frac{c_4 c_1 c_0^2}{1!1!2!} 
+ \frac{c_3 c_2 c_0^2}{1!1!2!} 
+ \frac{c_3 c_1^2 c_0}{1!2!1!}
+ \frac{c_2^2 c_1 c_0}{2!1!1!} 
+ \frac{c_2 c_1^3}{1!3!} \\
%
h_{(4,6)} &=
  \frac{c_6 c_0^3}{1!3!} 
+ \frac{c_5 c_1 c_0^2}{1!1!2!} 
+ \frac{c_4 c_2 c_0^2}{1!1!2!} 
+ \frac{c_4 c_1^2 c_0}{1!2!1!}
+ \frac{c_3^2 c_0^2}{2!2!} 
+ \frac{c_3 c_2 c_1 c_0}{1!1!1!1!} 
+ \frac{c_3 c_1^3}{1!3!} 
+ \frac{c_2^3 c_0}{3!1!}
+ \frac{c_2^2 c_1^2}{2!2!} \\
%
&\ldots
\end{aligned}  \right. \end{equation*}

\begin{equation*} \left| \begin{aligned}
h_{(5,0)} &=
  \frac{c_0^5}{5!} \\ 
%
h_{(5,1)} &=
  \frac{c_1 c_0^4}{1!4!} \\
%
h_{(5,2)} &=
  \frac{c_2 c_0^4}{1!4!} 
+ \frac{c_1^2 c_0^3}{2!3!} \\
%
h_{(5,3)} &=
  \frac{c_3 c_0^4}{1!4!} 
+ \frac{c_2 c_1 c_0^3}{1!1!3!} 
+ \frac{c_1^3 c_0^2}{3!2!} \\
%
h_{(5,4)} &=
  \frac{c_4 c_0^4}{1!4!} 
+ \frac{c_3 c_1 c_0^3}{1!1!3!} 
+ \frac{c_2^2 c_0^3}{2!3!}
+ \frac{c_2 c_1^2 c_0^2}{1!2!2!} 
+ \frac{c_1^4 c_0}{4!1!} \\
%
h_{(5,5)} &=
  \frac{c_5 c_0^4}{1!4!} 
+ \frac{c_4 c_1 c_0^3}{1!1!3!} 
+ \frac{c_3 c_2 c_0^3}{1!1!2!}
+ \frac{c_3 c_1^2 c_0^2}{1!2!2!} 
+ \frac{c_2^2 c_1 c_0^2}{2!1!2!} 
+ \frac{c_2 c_1^3 c_0}{1!3!1!} 
+ \frac{c_1^5}{5!} \\
%
h_{(5,6)} &=
  \frac{c_6 c_0^4}{1!4!} 
+ \frac{c_5 c_1 c_0^3}{1!1!3!} 
+ \frac{c_4 c_2 c_0^3}{1!1!3!}
+ \frac{c_4 c_1^2 c_0^2}{1!2!2!} 
+ \frac{c_3^2 c_0^3}{2!3!} 
+ \frac{c_3 c_2 c_1 c_0^2}{1!1!1!2!} 
+ \frac{c_3 c_1^3 c_0}{1!3!1!}
+ \frac{c_2^3 c_0^2}{3!2!} 
+ \frac{c_2^2 c_1^2 c_0}{2!2!1!} 
+ \frac{c_2 c_1^4}{1!4!} \\
%
&\ldots
\end{aligned} \right. \end{equation*}

\subsection{Показательная функция от многочлена}

\begin{equation*}
\begin{aligned}
C &= c_1 x + c_2 x^2 + c_3 x^3 + c_4 x^4 + \ldots \\
\exp{C} &= 1 + h_1 x + h_2 x^2 + h_3 x^3 + \ldots \\
\end{aligned}
\end{equation*}

\begin{equation*}
\left|
\begin{aligned} 
%---------------------------------------
h_1 
&= \frac{c_1}{1!} \\ 
%---------------------------------------
h_2 
&= \frac{c_2}{1!} 
+ \frac{c_1^2}{2!} \\
%---------------------------------------
h_3 
&= \frac{c_3}{1!} 
+ \frac{c_2 c_1}{1!1!} 
+ \frac{c_1^3}{3!} \\
%---------------------------------------
h_4 
&= \frac{c_4}{1!} 
+ \frac{c_3 c_1}{1!1!} 
+ \frac{c_2^2}{2!} 
+ \frac{c_2 c_1^2}{1!2!} 
+ \frac{c_1^4}{4!} \\
%---------------------------------------
h_5
&= \frac{c_5}{1!}
+ \frac{c_4 c_1}{1!1!}
+ \frac{c_3 c_2}{1!1!}
+ \frac{c_3 c_1^2}{1!2!}
+ \frac{c_2^2 c_1}{2!1!}
+ \frac{c_2 c_1^3}{1!3!}
+ \frac{c_1^5}{5!} \\
%---------------------------------------
&\ldots
\end{aligned}
\right.
\end{equation*}
