% !TeX root = sincotsec.tex

\subsection{Три разновидности оператора}

\begin{equation*}
P =
\left( 
\frac{1}{c_1},
\frac{1}{c_2}, 
\frac{1}{c_3}, 
{} \ldots, 
\frac{1}{c_n}
\right) 
\end{equation*}

\begin{equation*} \begin{aligned}
\mathrm{Z}_1(P) &= \mathrm{L}[1](P) \\
\mathrm{Z}_2(P) &= \mathrm{L}[2](P) \\
\mathrm{Z}_3(P) &= \mathrm{L}[3](P) \\
\mathrm{Z}_4(P) &= \mathrm{L}[4](P) \\
\mathrm{Z}_5(P) &= \mathrm{L}[5](P) \\
&\ldots \\
\end{aligned} \end{equation*}

\begin{equation*} \begin{aligned}
\Sigma_1(P) &= \mathrm{L}[1](P) \\
\Sigma_2(P) &= \mathrm{L}[1,1](P) \\
\Sigma_3(P) &= \mathrm{L}[1,1,1](P) \\
\Sigma_4(P) &= \mathrm{L}[1,1,1,1](P) \\
\Sigma_5(P) &= \mathrm{L}[1,1,1,1,1](P) \\
&\ldots \\
\end{aligned} \end{equation*}

\begin{equation*} \begin{aligned}
\mathrm{M}_1(P) &=
  \mathrm{L}[1](P) \\
%
\mathrm{M}_2(P) &=
  \mathrm{L}[2](P)
+ \mathrm{L}[1,1](P) \\
%
\mathrm{M}_3(P) &=
  \mathrm{L}[3](P)
+ \mathrm{L}[2,1](P)
+ \mathrm{L}[1,1,1](P) \\
%
\mathrm{M}_4(P) &=
  \mathrm{L}[4](P)
+ \mathrm{L}[3,1](P)
+ \mathrm{L}[2,2](P)
+ \mathrm{L}[2,1,1](P)
+ \mathrm{L}[1,1,1,1](P) \\
%
\mathrm{M}_5(P) &=
  \mathrm{L}[5](P)
+ \mathrm{L}[4,1](P)
+ \mathrm{L}[3,2](P)
+ \mathrm{L}[3,1,1](P)
+ \mathrm{L}[2,2,1](P)
+ \mathrm{L}[2,1,1,1](P) \\ &
+ \mathrm{L}[1,1,1,1,1](P) \\
%
\mathrm{M}_6(P) &=
  \mathrm{L}[6](P)
+ \mathrm{L}[5,1](P)
+ \mathrm{L}[4,2](P)
+ \mathrm{L}[4,1,1](P)
+ \mathrm{L}[3,3](P)
+ \mathrm{L}[3,2,1](P) \\ &
+ \mathrm{L}[3,1,1,1](P)
+ \mathrm{L}[2,2,2](P)
+ \mathrm{L}[2,2,1,1](P)
+ \mathrm{L}[2,1,1,1,1](P) \\ &
+ \mathrm{L}[1,1,1,1,1,1](P) \\
%
&\ldots \\
\end{aligned} \end{equation*}

\begin{equation*} \begin{aligned}
\zeta_1 &= \mathrm{Z}_1(P)
&
\sigma_1 &= \Sigma_1(P)
&
\mu_1 &= \mathrm{M}_1(P)
\\
\zeta_2 &= \mathrm{Z}_2(P)
&
\sigma_2 &= \Sigma_2(P)
&
\mu_2 &= \mathrm{M}_2(P)
\\
\zeta_3 &= \mathrm{Z}_3(P)
&
\sigma_3 &= \Sigma_3(P)
&
\mu_3 &= \mathrm{M}_3(P)
\\
\zeta_4 &= \mathrm{Z}_4(P)
&
\sigma_4 &= \Sigma_4(P)
&
\mu_4 &= \mathrm{M}_4(P)
\\
&\ldots
&
&\ldots
&
&\ldots
\\
\end{aligned} \end{equation*}

\begin{equation*} \begin{aligned}
\Delta(x) &=
  \frac{\zeta_1}{1} x
+ \frac{\zeta_2}{2} x^2
+ \frac{\zeta_3}{3} x^3
+ \frac{\zeta_4}{4} x^4
+ \ldots =
- \ln{
  \left[
  \left(1 - \frac{x}{c_1} \right)
  \left(1 - \frac{x}{c_2} \right)
  \left(1 - \frac{x}{c_3} \right)
  \cdot \ldots \cdot
  \left(1 - \frac{x}{c_n} \right)
  \right]
  } \\
%
\mathrm{M}(x) &=
  1
+ \mu_1 x
+ \mu_2 x^2
+ \mu_3 x^3
+ \ldots =
  \frac{1}{1 - \cfrac{x}{c_1}}
  \frac{1}{1 - \cfrac{x}{c_2}}
  \frac{1}{1 - \cfrac{x}{c_3}}
  \cdot \ldots \cdot
  \frac{1}{1 - \cfrac{x}{c_n}} \\
%
\Sigma(x) &=
  1
- \sigma_1 x
+ \sigma_2 x^2
- \sigma_3 x^3
+ \ldots =
  \left(1 - \frac{x}{c_1} \right)
  \left(1 - \frac{x}{c_2} \right)
  \left(1 - \frac{x}{c_3} \right)
  \cdot \ldots \cdot 
  \left(1 - \frac{x}{c_n} \right) \\
%
|x| &< |c_1| < |c_2| < |c_3| < \ldots < |c_n| \\
\end{aligned} \end{equation*}

\begin{equation*} \begin{aligned}
\mathrm{M}(x) &= \exp{\Delta(x)} = \frac{1}{\Sigma(x)} \\
\Sigma(x) &= \exp{(- \Delta(x))} = \frac{1}{\mathrm{M}(x)} \\
\Delta(x) &= \ln{\mathrm{M}(x)} = - \ln{\Sigma(x)} \\
\end{aligned} \end{equation*}

\begin{equation*} \left| \begin{aligned} 
\mu_1 &
= \frac{\zeta_1^1}{1!1^1} \\ 
%
\mu_2 &
= \frac{\zeta_2^1}{1!2^1} 
+ \frac{\zeta_1^2}{2!1^2} \\
%
\mu_3 &
= \frac{\zeta_3^1}{1!3^1} 
+ \frac{\zeta_2^1 \zeta_1^1}{1!2^1 \cdot 1!1^1} 
+ \frac{\zeta_1^3}{3!1^3} \\
%
\mu_4 &
= \frac{\zeta_4^1}{1!4^1} 
+ \frac{\zeta_3^1 \zeta_1^1}{1!3^1 \cdot 1!1^1} 
+ \frac{\zeta_2^2}{2!2^2} 
+ \frac{\zeta_2^1 \zeta_1^2}{1!2^1 \cdot 2!1^2} 
+ \frac{\zeta_1^4}{4!1^4} \\
%
\mu_5 &
= \frac{\zeta_5^1}{1!5^1}
+ \frac{\zeta_4^1 \zeta_1^1}{1!4^1 \cdot 1!1^1}
+ \frac{\zeta_3^1 \zeta_2^1}{1!3^1 \cdot 1!2^1}
+ \frac{\zeta_3^1 \zeta_1^2}{1!3^1 \cdot 2!1^2}
+ \frac{\zeta_2^2 \zeta_1^1}{2!2^2 \cdot 1!1^1}
+ \frac{\zeta_2^1 \zeta_1^3}{1!2^1 \cdot 3!1^3}
+ \frac{\zeta_1^5}{5!1^5} \\
%
&\ldots
\end{aligned} \right. \end{equation*}

\begin{equation*} \left| \begin{aligned} 
\sigma_1 &=
  \frac{\zeta_1^1}{1!1^1}
\\ 
\sigma_2 &=
- \frac{\zeta_2^1}{1!2^1} 
+ \frac{\zeta_1^2}{2!1^2}
\\
\sigma_3 &=
  \frac{\zeta_3^1}{1!3^1} 
- \frac{\zeta_2^1 \zeta_1^1}{1!2^1 \cdot 1!1^1} 
+ \frac{\zeta_1^3}{3!1^3}
\\
\sigma_4 &=
- \frac{\zeta_4^1}{1!4^1} 
+ \frac{\zeta_3^1 \zeta_1^1}{1!3^1 \cdot 1!1^1} 
+ \frac{\zeta_2^2}{2!2^2} 
- \frac{\zeta_2^1 \zeta_1^2}{1!2^1 \cdot 2!1^2} 
+ \frac{\zeta_1^4}{4!1^4}
\\
\sigma_5 &=
  \frac{\zeta_5^1}{1!5^1}
- \frac{\zeta_4^1 \zeta_1^1}{1!4^1 \cdot 1!1^1}
- \frac{\zeta_3^1 \zeta_2^1}{1!3^1 \cdot 1!2^1}
+ \frac{\zeta_3^1 \zeta_1^2}{1!3^1 \cdot 2!1^2}
+ \frac{\zeta_2^2 \zeta_1^1}{2!2^2 \cdot 1!1^1}
- \frac{\zeta_2^1 \zeta_1^3}{1!2^1 \cdot 3!1^3}
+ \frac{\zeta_1^5}{5!1^5}
\\
&\ldots
\\
\end{aligned} \right. \end{equation*}

\begin{equation*} \left| \begin{aligned}
\sigma_1 &= 
  \frac{1!}{0!} \frac{\mu_1^1}{1!}
\\ 
\sigma_2 &= 
- \frac{1!}{0!} \frac{\mu_2^1}{1!} 
+ \frac{2!}{0!} \frac{\mu_1^2}{2!}
\\
\sigma_3 &= 
  \frac{1!}{0!} \frac{\mu_3^1}{1!} 
- \frac{2!}{0!} \frac{\mu_2^1 \mu_1}{1!1!} 
+ \frac{3!}{0!} \frac{\mu_1^3}{3!}
\\
\sigma_4 &= 
- \frac{1!}{0!} \frac{\mu_4^1}{1!} 
+ \frac{2!}{0!} \frac{\mu_3^1 \mu_1^1}{1!1!} 
+ \frac{2!}{0!} \frac{\mu_2^2}{2!}
- \frac{3!}{0!} \frac{\mu_2^1 \mu_1^2}{1!2!}
+ \frac{4!}{0!} \frac{\mu_1^4}{4!}
\\
\sigma_5 &=
  \frac{1!}{0!} \frac{\mu_5^1}{1!} 
- \frac{2!}{0!} \frac{\mu_4^1 \mu_1^1}{1!1!} 
- \frac{2!}{0!} \frac{\mu_3^1 \mu_2^1}{1!1!}
+ \frac{3!}{0!} \frac{\mu_3^1 \mu_1^2}{1!2!}
+ \frac{3!}{0!} \frac{\mu_2^2 \mu_1^1}{2!1!}
- \frac{4!}{0!} \frac{\mu_2^1 \mu_1^3}{1!3!}
+ \frac{5!}{0!} \frac{\mu_1^5}{5!}
\\
\sigma_6 &=
- \frac{1!}{0!} \frac{\mu_6^1}{1!} 
+ \frac{2!}{0!} \frac{\mu_5^1 \mu_1^1}{1!1!} 
+ \frac{2!}{0!} \frac{\mu_4^1 \mu_2^1}{1!1!}
- \frac{3!}{0!} \frac{\mu_4^1 \mu_1^2}{1!2!}
+ \frac{2!}{0!} \frac{\mu_3^2}{2!}
- \frac{3!}{0!} \frac{\mu_3^1 \mu_2^1 \mu_1^1}{1!1!1!}
+ \frac{4!}{0!} \frac{\mu_3^1 \mu_1^3}{1!3!}
- \frac{3!}{0!} \frac{\mu_2^3}{3!}
+ \frac{4!}{0!} \frac{\mu_2^2 \mu_1^2}{2!2!} \\
&
- \frac{5!}{0!} \frac{\mu_2^1 \mu_1^4}{1!4!}
+ \frac{6!}{0!} \frac{\mu_1^6}{6!}
\\
&\ldots
\\
\end{aligned} \right. \end{equation*}

\begin{equation*} \left| \begin{aligned}
\mu_1 &= 
  \frac{1!}{0!} \frac{\sigma_1^1}{1!}
\\
\mu_2 &= 
- \frac{1!}{0!} \frac{\sigma_2^1}{1!} 
+ \frac{2!}{0!} \frac{\sigma_1^2}{2!}
\\
\mu_3 &= 
  \frac{1!}{0!} \frac{\sigma_3^1}{1!} 
- \frac{2!}{0!} \frac{\sigma_2^1 \sigma_1^1}{1!1!} 
+ \frac{3!}{0!} \frac{\sigma_1^3}{3!}
\\
\mu_4 &= 
- \frac{1!}{0!} \frac{\sigma_4^1}{1!} 
+ \frac{2!}{0!} \frac{\sigma_3^1 \sigma_1^1}{1!1!} 
+ \frac{2!}{0!} \frac{\sigma_2^2}{2!}
- \frac{3!}{0!} \frac{\sigma_2^1 \sigma_1^2}{1!2!}
+ \frac{4!}{0!} \frac{\sigma_1^4}{4!}
\\
\mu_5 &=
  \frac{1!}{0!} \frac{\sigma_5^1}{1!} 
- \frac{2!}{0!} \frac{\sigma_4^1 \sigma_1^1}{1!1!} 
- \frac{2!}{0!} \frac{\sigma_3^1 \sigma_2^1}{1!1!}
+ \frac{3!}{0!} \frac{\sigma_3^1 \sigma_1^2}{1!2!}
+ \frac{3!}{0!} \frac{\sigma_2^2 \sigma_1^1}{2!1!}
- \frac{4!}{0!} \frac{\sigma_2^1 \sigma_1^3}{1!3!}
+ \frac{5!}{0!} \frac{\sigma_1^5}{5!}
\\
\mu_6 &=
- \frac{1!}{0!} \frac{\sigma_6^1}{1!} 
+ \frac{2!}{0!} \frac{\sigma_5^1 \sigma_1^1}{1!1!} 
+ \frac{2!}{0!} \frac{\sigma_4^1 \sigma_2^1}{1!1!}
- \frac{3!}{0!} \frac{\sigma_4^1 \sigma_1^2}{1!2!}
+ \frac{2!}{0!} \frac{\sigma_3^2}{2!}
- \frac{3!}{0!} \frac{\sigma_3^1 \sigma_2^1 \sigma_1^1}{1!1!1!}
+ \frac{4!}{0!} \frac{\sigma_3^1 \sigma_1^3}{1!3!}
- \frac{3!}{0!} \frac{\sigma_2^3}{3!}
+ \frac{4!}{0!} \frac{\sigma_2^2 \sigma_1^2}{2!2!} \\ &
- \frac{5!}{0!} \frac{\sigma_2^1 \sigma_1^4}{1!4!}
+ \frac{6!}{0!} \frac{\sigma_1^6}{6!}
\\
&\ldots
\\
\end{aligned} \right. \end{equation*}