% !TeX root = sincotsec.tex

\section{Суммы значений $\omega$-функций}

\subsection{$\omega_0$-функции}

\begin{equation*} \begin{aligned}
\slf_0(x) &=
  \frac{1^0}{0!} 
+ \frac{2^0}{0!} 
+ \frac{3^0}{0!} 
+ \frac{4^0}{0!} 
+ \ldots 
+ \frac{x^0}{0!} \\
%
\slf_1(x) &= 
  \frac{1^1}{1!} 
+ \frac{2^1}{1!} 
+ \frac{3^1}{1!} 
+ \frac{4^1}{1!} 
+ \ldots 
+ \frac{x^1}{1!} \\
%
\slf_2(x) &= 
  \frac{1^2}{2!} 
+ \frac{2^2}{2!} 
+ \frac{3^2}{2!} 
+ \frac{4^2}{2!} 
+ \ldots 
+ \frac{x^2}{2!} \\
%
\slf_3(x) &= 
  \frac{1^3}{3!} 
+ \frac{2^3}{3!} 
+ \frac{3^3}{3!} 
+ \frac{4^3}{3!} 
+ \ldots 
+ \frac{x^3}{3!} \\
%
&\ldots \\
\end{aligned} \end{equation*}

\begin{equation*} \begin{aligned}
\slf_0(x + 1) &= 
  \slf_0(x) + \elf_0(x + 1)
\\
\slf_1(x + 1) &= 
  \slf_1(x) + \elf_1(x + 1)  
\\
\slf_2(x + 1) &= 
  \slf_2(x) + \elf_2(x + 1)  
\\
\slf_3(x + 1) &= 
  \slf_3(x) + \elf_3(x + 1)  
\\
\slf_4(x + 1) &= 
  \slf_4(x) + \elf_4(x + 1)  
\\
&\ldots \\
\end{aligned} \end{equation*}

\begin{equation*} \begin{aligned}
\mathrm{D}_1 \left[\slf_0(x + 1) - \slf_0(x) \right] &= 0
\\
\mathrm{D}_1 \left[\slf_1(x + 1) - \slf_1(x) \right] &= \slf_0(x + 1) - \slf_0(x)  
\\
\mathrm{D}_1 \left[\slf_2(x + 1) - \slf_2(x) \right] &= \slf_1(x + 1) - \slf_1(x)  
\\
\mathrm{D}_1 \left[\slf_3(x + 1) - \slf_3(x) \right] &= \slf_2(x + 1) - \slf_2(x)  
\\
\mathrm{D}_1 \left[\slf_4(x + 1) - \slf_4(x) \right] &= \slf_3(x + 1) - \slf_3(x)  
\\
&\ldots \\
\end{aligned} \end{equation*}

\begin{equation*} \begin{aligned}
\mathrm{D}_1 \slf_0(x) &= t_0  
\\
\mathrm{D}_1 \slf_1(x) &= \slf_0(x) + t_1  
\\
\mathrm{D}_1 \slf_2(x) &= \slf_1(x) + t_2  
\\
\mathrm{D}_1 \slf_3(x) &= \slf_2(x) + t_3 
\\
\mathrm{D}_1 \slf_4(x) &= \slf_3(x) + t_4 
\\
&\ldots
\\
\end{aligned} \end{equation*}

\begin{equation*} \begin{aligned}
\slf_0(0) &= 0 & \slf_0(1) &= \elf_0(1)
\\
\slf_1(0) &= 0 & \slf_1(1) &= \elf_1(1)
\\
\slf_2(0) &= 0 & \slf_2(1) &= \elf_2(1)
\\
\slf_3(0) &= 0 & \slf_3(1) &= \elf_3(1)
\\
\slf_4(0) &= 0 & \slf_4(1) &= \elf_4(1)
\\
&\ldots & &\ldots
\\
\end{aligned} \end{equation*}

\begin{equation*} \begin{aligned}
\slf_0(x) &= 
  t_0 \frac{x}{1!} 
\\
\slf_1(x) &= 
  t_1 \frac{x}{1!} 
+ t_0 \frac{x^2}{2!} 
\\
\slf_2(x) &= 
  t_2 \frac{x}{1!} 
+ t_1 \frac{x^2}{2!} 
+ t_0 \frac{x^3}{3!} 
\\
\slf_3(x) &= 
  t_3 \frac{x}{1!} 
+ t_2 \frac{x^2}{2!} 
+ t_1 \frac{x^3}{3!} 
+ t_0 \frac{x^4}{4!} 
\\
&\ldots
\\
\end{aligned} \end{equation*}

\begin{equation*} \begin{aligned}
  t_0
+ t_1 x
+ t_2 x^2
+ t_3 x^3
+ \ldots
&
= \frac{x \exp{x}}{\exp{x} - 1}
= \frac{x}{2} \coth{\frac{x}{2}} 
+ \frac{x}{2}
\\
\end{aligned} \end{equation*}

\subsection{$\omega_1$-функции}

\begin{equation*} \begin{aligned}
&\ldots
\\
\slg_{-3}(x) &=
  \frac{2!}{1^3}
+ \frac{2!}{2^3} 
+ \frac{2!}{3^3} 
+ \ldots 
+ \frac{2!}{x^3}
\\
\slg_{-2}(x) &=
- \frac{1!}{1^2}
- \frac{1!}{2^2} 
- \frac{1!}{3^2} 
+ \ldots 
- \frac{1!}{x^2}
\\
\slg_{-1}(x) &=
  \frac{0!}{1^1}
+ \frac{0!}{2^1} 
+ \frac{0!}{3^1} 
+ \ldots 
+ \frac{0!}{x^1}
\\
\slg_0(x) &=
  \left( \frac{1^0}{0!} \ln{1} - \Theta_0 \frac{1^0}{0!} \right)
+ \left( \frac{2^0}{0!} \ln{2} - \Theta_0 \frac{2^0}{0!} \right) 
+ \left( \frac{3^0}{0!} \ln{3} - \Theta_0 \frac{3^0}{0!} \right) 
+ \ldots 
+ \left( \frac{x^0}{0!} \ln{x} - \Theta_0 \frac{x^0}{0!} \right)
\\
\slg_1(x) &=
  \left(\frac{1^1}{1!} \ln{1} - \Theta_1 \frac{1^1}{1!} \right)
+ \left( \frac{2^1}{1!} \ln{2} - \Theta_1 \frac{2^1}{1!} \right) 
+ \left( \frac{3^1}{1!} \ln{3} - \Theta_1 \frac{3^1}{1!} \right) 
+ \ldots 
+ \left( \frac{x^1}{1!} \ln{x} - \Theta_1 \frac{x^1}{1!} \right)
\\
\slg_2(x) &=
  \left( \frac{1^2}{2!} \ln{1} - \Theta_2 \frac{1^2}{2!} \right)
+ \left( \frac{2^2}{2!} \ln{2} - \Theta_2 \frac{2^2}{2!} \right) 
+ \left( \frac{3^2}{2!} \ln{3} - \Theta_2 \frac{3^2}{2!} \right) 
+ \ldots 
+ \left( \frac{x^2}{2!} \ln{x} - \Theta_2 \frac{x^2}{2!} \right)
\\
&\ldots
\\
\end{aligned} \end{equation*}

\begin{equation*} \begin{aligned}
&\ldots
\\
\slg_{-2}(x + 1) &= 
  \slg_{-2}(x) + \elg_{-2}(x + 1)
\\
\slg_{-1}(x + 1) &= 
  \slg_{-1}(x) + \elg_{-1}(x + 1)
\\
\slg_0(x + 1) &= 
  \slg_0(x) + \elg_0(x + 1)
\\
\slg_1(x + 1) &= 
  \slg_1(x) + \elg_1(x + 1)  
\\
\slg_2(x + 1) &= 
  \slg_2(x) + \elg_2(x + 1)
\\
&\ldots
\\
\end{aligned} \end{equation*}

\begin{equation*} \begin{aligned}
&\ldots
\\
\mathrm{D}_1 \left[\slg_{-2}(x + 1) - \slg_{-2}(x) \right] &= \slg_{-3}(x + 1) - \slg_{-3}(x)  
\\
\mathrm{D}_1 \left[\slg_{-1}(x + 1) - \slg_{-1}(x) \right] &= \slg_{-2}(x + 1) - \slg_{-2}(x)  
\\
\mathrm{D}_1 \left[\slg_0(x + 1) - \slg_0(x) \right] &= \slg_{-1}(x + 1) - \slg_{-1}(x)  
\\
\mathrm{D}_1 \left[\slg_1(x + 1) - \slg_1(x) \right] &= \slg_0(x + 1) - \slg_0(x)  
\\
\mathrm{D}_1 \left[\slg_2(x + 1) - \slg_2(x) \right] &= \slg_1(x + 1) - \slg_1(x)  
\\
&\ldots
\\
\end{aligned} \end{equation*}

\begin{equation*} \begin{aligned}
&\ldots
\\
\mathrm{D}_1 \slg_{-2}(x) &= \slg_{-3}(x) + u_{-2}  
\\
\mathrm{D}_1 \slg_{-1}(x) &= \slg_{-2}(x) + u_{-1}  
\\
\mathrm{D}_1 \slg_0(x) &= \slg_{-1}(x) + u_0  
\\
\mathrm{D}_1 \slg_1(x) &= \slg_0(x) + u_1  
\\
\mathrm{D}_1 \slg_2(x) &= \slg_1(x) + u_2
\\
&\ldots
\\
\end{aligned} \end{equation*}