% !TeX root = sincotsec.tex

\section{Производная}

\begin{equation*}
\begin{aligned}
T_1(x,a) &= 
  \frac{1!}{1!0!} f(x + a) 
- \frac{1!}{0!1!} f(x)
\\
T_2(x,a) &= 
  \frac{2!}{2!0!} f(x + 2 a) 
- \frac{2!}{1!1!} f(x + a) 
+ \frac{2!}{0!2!} f(x)
\\
T_3(x,a) &=
  \frac{3!}{3!0!} f(x + 3 a) 
- \frac{3!}{2!1!} f(x + 2 a) 
+ \frac{3!}{1!2!} f(x + a)
- \frac{3!}{0!3!} f(x)
\\
T_4(x,a) &= 
  \frac{4!}{4!0!} f(x + 4 a) 
- \frac{4!}{3!1!} f(x + 3 a) 
+ \frac{4!}{2!2!} f(x + 2 a) 
- \frac{4!}{1!3!} f(x + a) 
+ \frac{4!}{0!4!} f(x)
\\
&\ldots
\\
\end{aligned}
\end{equation*}

\begin{equation*}
\begin{aligned}
\mathrm{D}_1 f(x) &= \lim_{a \to 0} \frac{T_1(x,a)}{a} \\
%
\mathrm{D}_2 f(x) &= \lim_{a \to 0} \frac{T_2(x,a)}{a^2} \\
%
\mathrm{D}_3 f(x) &= \lim_{a \to 0} \frac{T_3(x,a)}{a^3} \\
%
\mathrm{D}_4 f(x) &= \lim_{a \to 0} \frac{T_4(x,a)}{a^4} \\
%
&\ldots \\
\end{aligned}
\end{equation*}

\begin{equation*}
\begin{aligned}
\mathrm{D}_{(1,0)} F(x, y) &=
\lim_{a \to 0}{\frac{
  F(x + a, y)
- F(x, y)
}{a}}
\\
\mathrm{D}_{(2,0)} F(x, y) &=
\lim_{a \to 0}{\frac{
  F(x + 2 a, y)
- 2 F(x + a, y)
+ F(x)
}{a^2}}
\\
\mathrm{D}_{(0,1)} F(x, y) &=
\lim_{a \to 0}{\frac{
  F(x, y + a)
- F(x, y)
}{a}}
\\
\mathrm{D}_{(1,1)} F(x, y) &=
\lim_{a \to 0}{\frac{{
  F(x + a, y + a)
- F(x, y + a)
- F(x + a, y)
+ F(x, y)
}}{a^2}}
\\
\end{aligned}
\end{equation*}
