% !TeX root = ../Collection.tex

\subsection{$\omega$-функции от $1 + x$}

\begin{equation*}
\begin{aligned}
\frac{(1 + x)^0}{0!} &=
  \frac{1}{0!0!} 
\\
\frac{(1 + x)^1}{1!} &=
  \frac{1}{1!0!} 
+ \frac{1}{0!1!} x
\\
\frac{(1 + x)^2}{2!} &= 
  \frac{1}{2!0!} 
+ \frac{1}{1!1!} x 
+ \frac{1}{0!2!} x^2
\\
\frac{(1 + x)^3}{3!} &=
  \frac{1}{3!0!} 
+ \frac{1}{2!1!} x 
+ \frac{1}{1!2!} x^2 
+ \frac{1}{0!3!} x^3
\\
\frac{(1 + x)^4}{4!} &=
  \frac{1}{4!0!} 
+ \frac{1}{3!1!} x 
+ \frac{1}{2!2!} x^2 
+ \frac{1}{1!3!} x^3 
+ \frac{1}{0!4!} x^4
\\
\frac{(1 + x)^5}{5!} &=
  \frac{1}{5!0!} 
+ \frac{1}{4!1!} x 
+ \frac{1}{3!2!} x^2 
+ \frac{1}{2!3!} x^3 
+ \frac{1}{1!4!} x^4
+ \frac{1}{0!5!} x^5
\\
&\ldots
\\
\end{aligned}
\end{equation*}

\begin{equation*}
\begin{aligned}
(1 + x)^1 &=
  \frac{1!}{1!0!} 
+ \frac{1!}{0!1!} x
\\
(1 + x)^2 &= 
  \frac{2!}{2!0!} 
+ \frac{2!}{1!1!} x 
+ \frac{2!}{0!2!} x^2
\\
(1 + x)^3 &=
  \frac{3!}{3!0!} 
+ \frac{3!}{2!1!} x 
+ \frac{3!}{1!2!} x^2 
+ \frac{3!}{0!3!} x^3
\\
(1 + x)^4 &=
  \frac{4!}{4!0!} 
+ \frac{4!}{3!1!} x 
+ \frac{4!}{2!2!} x^2 
+ \frac{4!}{1!3!} x^3 
+ \frac{4!}{0!4!} x^4
\\
(1 + x)^5 &=
  \frac{5!}{5!0!} 
+ \frac{5!}{4!1!} x 
+ \frac{5!}{3!2!} x^2 
+ \frac{5!}{2!3!} x^3 
+ \frac{5!}{1!4!} x^4
+ \frac{5!}{0!5!} x^5
\\
&\ldots
\\
\end{aligned}
\end{equation*}

\begin{equation*} \begin{aligned}
&\ldots \\
%
- \frac{1}{(1 + x)^2} &= 
- \frac{1!}{0!} x^{-2}
+ \frac{2!}{1!} x^{-3}
- \frac{3!}{2!} x^{-4}
+ \frac{4!}{3!} x^{-5}
- \frac{5!}{4!} x^{-6}
+ \frac{6!}{5!} x^{-7}
+ \ldots & 
&|x| > 1 \\
%
  \frac{1}{1 + x} &=  
  \frac{0!}{0!} x^{-1}
- \frac{1!}{1!} x^{-2}
+ \frac{2!}{2!} x^{-3}
- \frac{3!}{3!} x^{-4}
+ \frac{4!}{4!} x^{-5}
- \frac{5!}{5!} x^{-6}
+ \ldots & 
&|x| > 1 \\
%
  \ln(1 + x) &=
  \ln{x}
+ \frac{0!}{1!} x^{-1} 
- \frac{1!}{2!} x^{-2}
+ \frac{2!}{3!} x^{-3}
- \frac{3!}{4!} x^{-4}
+ \frac{4!}{5!} x^{-5}
+ \ldots & 
&|x| > 1 \\
%
&\ldots \\
\end{aligned} \end{equation*}
%
\begin{equation*} \begin{aligned}
&\ldots \\
%
- \frac{1}{(1 + x)^2} &= 
- \frac{1!}{0!}
+ \frac{2!}{1!} x
- \frac{3!}{2!} x^2
+ \frac{4!}{3!} x^3
- \frac{5!}{4!} x^4
+ \frac{6!}{5!} x^5
+ \ldots & 
&|x| < 1 \\
%
  \frac{1}{1 + x} &=  
  \frac{0!}{0!}
- \frac{1!}{1!} x
+ \frac{2!}{2!} x^2
- \frac{3!}{3!} x^3
+ \frac{4!}{4!} x^4
- \frac{5!}{5!} x^5
+ \ldots & 
&|x| < 1 \\
%
  \ln(1 + x) &=
  \ln{1}
+ \frac{0!}{1!} x 
- \frac{1!}{2!} x^2
+ \frac{2!}{3!} x^3
- \frac{3!}{4!} x^4
+ \frac{4!}{5!} x^5
+ \ldots & 
&|x| < 1 \\
%
&\ldots \\
\end{aligned} \end{equation*}
