% !TeX root = sincotsec.tex

\section{$\omega$-функции}

\subsection{$\omega_0$-функции}

\begin{equation*}\begin{aligned}
&\ldots \\
\omega_{(0,0)}(x) &= \frac{x^0}{0!} \\
\omega_{(0,1)}(x) &= \frac{x^1}{1!} \\
\omega_{(0,2)}(x) &= \frac{x^2}{2!} \\
\omega_{(0,3)}(x) &= \frac{x^3}{3!} \\
\omega_{(0,4)}(x) &= \frac{x^4}{4!} \\
&\ldots \\
\end{aligned}\end{equation*}

\begin{equation*}
\lim_{p \to 0} \frac{\omega_{(0, n)}(x + p) - \omega_{(0, n)}(x)}{p} = \omega_{(0, n - 1)}(x) \\
\end{equation*}

\subsection{$\omega_1$-функции}

\begin{equation*} \begin{aligned}
&\ldots \\
\omega_{(1, -4)}(x) &=
- \frac{3!}{x^4} \\
\omega_{(1, -3)}(x) &=
  \frac{2!}{x^3} \\
\omega_{(1, -2)}(x) &=
- \frac{1!}{x^2} \\
\omega_{(1, -1)}(x) &=
  \frac{0!}{x^1} \\
\omega_{(1, 0)}(x) &= 
  \frac{x^0}{0!} \left(
  \ln{x} - \Theta_0 \right) \\
\omega_{(1, 1)}(x) &= 
  \frac{x^1}{1!} \left(
  \ln{x} - \Theta_1 \right) \\
\omega_{(1, 2)}(x) &= 
  \frac{x^2}{2!} \left(
  \ln{x} - \Theta_2 \right) \\
\omega_{(1, 3)}(x) &= 
  \frac{x^3}{3!} \left(
  \ln{x} - \Theta_3 \right) \\
\omega_{(1, 4)}(x) &= 
  \frac{x^4}{4!} \left(
  \ln{x} - \Theta_4 \right) \\
&\ldots \\
\end{aligned} \end{equation*}

\begin{equation*} \begin{aligned}
\Theta_0 &= 0 \\
\Theta_1 &= 
  \frac{1}{1} \\
\Theta_2 &= 
  \frac{1}{1} 
+ \frac{1}{2} \\
\Theta_3 &= 
  \frac{1}{1} 
+ \frac{1}{2} 
+ \frac{1}{3} \\
\Theta_4 &= 
  \frac{1}{1} 
+ \frac{1}{2} 
+ \frac{1}{3} 
+ \frac{1}{4} \\
&\ldots \\
\end{aligned} \end{equation*}

\begin{equation*}
\lim_{p \to 0} \frac{\omega_{(1, n)}(x + p) - \omega_{(1, n)}(x)}{p} = \omega_{(1, n - 1)}(x) \\
\end{equation*}
