% !TeX root = ../Collection.tex

\subsection{$\omega$-функции от многочлена}

\begin{equation*}
C(x) = c_0 + c_1 x + c_2 x^2 + c_3 x^3 + c_4 x^4 + \ldots \\
\end{equation*}

\begin{equation*}\begin{aligned}
\omega_{N}(C) &= \sum_{i_0 + i_1 + \ldots = N}
{
  \omega_{i_0}(c_0 x^0)
  \omega_{i_1}(c_1 x^1)
  \omega_{i_2}(c_2 x^2)
  \cdot
  \ldots
} \\
&= \sum_{i_0 + i_1 + \ldots = N}
{
  \frac{c_0^{i_0} c_1^{i_1} c_2^{i_2} \cdot \ldots}{i_0! i_1! i_2! \cdot \ldots}
  x^{[0 i_0 + 1 i_1 + 2 i_2 + \ldots]}
} \\
\end{aligned}\end{equation*}

\begin{equation*} \begin{aligned}
\omega_{0}(C) &= h_{(0,0)} + h_{(0,1)} x + h_{(0,2)} x^2 + h_{(0,3)} x^3 + \ldots \\
\omega_{1}(C) &= h_{(1,0)} + h_{(1,1)} x + h_{(1,2)} x^2 + h_{(1,3)} x^3 + \ldots \\
\omega_{2}(C) &= h_{(2,0)} + h_{(2,1)} x + h_{(2,2)} x^2 + h_{(2,3)} x^3 + \ldots \\
\omega_{3}(C) &= h_{(3,0)} + h_{(3,1)} x + h_{(3,2)} x^2 + h_{(3,3)} x^3 + \ldots \\
\omega_{4}(C) &= h_{(4,0)} + h_{(4,1)} x + h_{(4,2)} x^2 + h_{(4,3)} x^3 + \ldots \\
\omega_{5}(C) &= h_{(5,0)} + h_{(5,1)} x + h_{(5,2)} x^2 + h_{(5,3)} x^3 + \ldots \\
&\ldots \\
\end{aligned} \end{equation*}

\begin{equation*} \left| \begin{aligned} 
h_{(0,0)} &= 1 \\ 
h_{(0,1)} &= 0 \\
h_{(0,2)} &= 0 \\
h_{(0,3)} &= 0 \\
h_{(0,4)} &= 0 \\
h_{(0,5)} &= 0 \\
h_{(0,6)} &= 0 \\
&\ldots
\end{aligned} \right. \end{equation*}

\begin{equation*} \left| \begin{aligned} 
h_{(1,0)} &= \frac{c_0}{1!} \\ 
h_{(1,1)} &= \frac{c_1}{1!} \\
h_{(1,2)} &= \frac{c_2}{1!} \\
h_{(1,3)} &= \frac{c_3}{1!} \\
h_{(1,4)} &= \frac{c_4}{1!} \\
h_{(1,5)} &= \frac{c_5}{1!} \\
h_{(1,6)} &= \frac{c_6}{1!} \\
&\ldots
\end{aligned} \right. \end{equation*}

\begin{equation*} \left| \begin{aligned} 
h_{(2,0)} &=
  \frac{c_0^2}{2!} \\
%
h_{(2,1)} &=
  \frac{c_1 c_0}{1!1!} \\
%
h_{(2,2)} &=
  \frac{c_2 c_0}{1!1!}
+ \frac{c_1^2}{2!} \\
%
h_{(2,3)} &=
  \frac{c_3 c_0}{1!1!}
+ \frac{c_2 c_1}{1!1!} \\
%
h_{(2,4)} &=
  \frac{c_4 c_0}{1!1!}
+ \frac{c_3 c_1}{1!1!}
+ \frac{c_2^2}{2!} \\
%
h_{(2,5)} &=
  \frac{c_5 c_0}{1!1!}
+ \frac{c_4 c_1}{1!1!}
+ \frac{c_3 c_2}{1!1!} \\
%
h_{(2,6)} &=
  \frac{c_6 c_0}{1!1!}
+ \frac{c_5 c_1}{1!1!}
+ \frac{c_4 c_2}{1!1!}
+ \frac{c_3^2}{2!} \\
%
&\ldots
\end{aligned} \right. \end{equation*}

\begin{equation*} \left| \begin{aligned}
h_{(3,0)} &=
  \frac{c_0^3}{3!} \\ 
%
h_{(3,1)} &=
  \frac{c_1 c_0^2}{1!2!} \\
%
h_{(3,2)} &=
  \frac{c_2 c_0^2}{1!2!} 
+ \frac{c_1^2 c_0}{2!1!} \\
%
h_{(3,3)} &=
  \frac{c_3 c_0^2}{1!2!} 
+ \frac{c_2 c_1 c_0}{1!1!1!} 
+ \frac{c_1^3}{3!} \\
%
h_{(3,4)} &=
  \frac{c_4 c_0^2}{1!2!} 
+ \frac{c_3 c_1 c_0}{1!1!1!} 
+ \frac{c_2^2 c_0}{2!1!} 
+ \frac{c_2 c_1^2}{1!2!} \\
%
h_{(3,5)} &=
  \frac{c_5 c_0^2}{1!2!} 
+ \frac{c_4 c_1 c_0}{1!1!1!} 
+ \frac{c_3 c_2 c_0}{1!1!1!} 
+ \frac{c_3 c_1^2}{1!2!}
+ \frac{c_2^2 c_1}{2!1!} \\
%
h_{(3,6)} &=
  \frac{c_6 c_0^2}{1!2!} 
+ \frac{c_5 c_1 c_0}{1!1!1!} 
+ \frac{c_4 c_2 c_0}{1!1!1!} 
+ \frac{c_4 c_1^2}{1!2!}
+ \frac{c_3^2 c_0}{2!1!} 
+ \frac{c_3 c_2 c_1}{1!1!1!} 
+ \frac{c_2^3}{3!} \\
%
&\ldots
\end{aligned} \right. \end{equation*}

\begin{equation*} \left| \begin{aligned} 
h_{(4,0)} &=
  \frac{c_0^4}{4!} \\ 
%
h_{(4,1)} &=
  \frac{c_1 c_0^3}{1!3!} \\
%
h_{(4,2)} &=
  \frac{c_2 c_0^3}{1!3!} 
+ \frac{c_1^2 c_0^2}{2!2!} \\
%
h_{(4,3)} &=
  \frac{c_3 c_0^3}{1!3!} 
+ \frac{c_2 c_1 c_0^2}{1!1!2!} 
+ \frac{c_1^3 c_0}{3!1!} \\
%
h_{(4,4)} &=
  \frac{c_4 c_0^3}{1!3!} 
+ \frac{c_3 c_1 c_0^2}{1!1!2!} 
+ \frac{c_2^2 c_0^2}{2!2!}
+ \frac{c_2 c_1^2 c_0}{1!2!1!} 
+ \frac{c_1^4}{4!} \\
%
h_{(4,5)} &=
  \frac{c_5 c_0^3}{1!3!} 
+ \frac{c_4 c_1 c_0^2}{1!1!2!} 
+ \frac{c_3 c_2 c_0^2}{1!1!2!} 
+ \frac{c_3 c_1^2 c_0}{1!2!1!}
+ \frac{c_2^2 c_1 c_0}{2!1!1!} 
+ \frac{c_2 c_1^3}{1!3!} \\
%
h_{(4,6)} &=
  \frac{c_6 c_0^3}{1!3!} 
+ \frac{c_5 c_1 c_0^2}{1!1!2!} 
+ \frac{c_4 c_2 c_0^2}{1!1!2!} 
+ \frac{c_4 c_1^2 c_0}{1!2!1!}
+ \frac{c_3^2 c_0^2}{2!2!} 
+ \frac{c_3 c_2 c_1 c_0}{1!1!1!1!} 
+ \frac{c_3 c_1^3}{1!3!} 
+ \frac{c_2^3 c_0}{3!1!}
+ \frac{c_2^2 c_1^2}{2!2!} \\
%
&\ldots
\end{aligned}  \right. \end{equation*}

\begin{equation*} \left| \begin{aligned}
h_{(5,0)} &=
  \frac{c_0^5}{5!} \\ 
%
h_{(5,1)} &=
  \frac{c_1 c_0^4}{1!4!} \\
%
h_{(5,2)} &=
  \frac{c_2 c_0^4}{1!4!} 
+ \frac{c_1^2 c_0^3}{2!3!} \\
%
h_{(5,3)} &=
  \frac{c_3 c_0^4}{1!4!} 
+ \frac{c_2 c_1 c_0^3}{1!1!3!} 
+ \frac{c_1^3 c_0^2}{3!2!} \\
%
h_{(5,4)} &=
  \frac{c_4 c_0^4}{1!4!} 
+ \frac{c_3 c_1 c_0^3}{1!1!3!} 
+ \frac{c_2^2 c_0^3}{2!3!}
+ \frac{c_2 c_1^2 c_0^2}{1!2!2!} 
+ \frac{c_1^4 c_0}{4!1!} \\
%
h_{(5,5)} &=
  \frac{c_5 c_0^4}{1!4!} 
+ \frac{c_4 c_1 c_0^3}{1!1!3!} 
+ \frac{c_3 c_2 c_0^3}{1!1!2!}
+ \frac{c_3 c_1^2 c_0^2}{1!2!2!} 
+ \frac{c_2^2 c_1 c_0^2}{2!1!2!} 
+ \frac{c_2 c_1^3 c_0}{1!3!1!} 
+ \frac{c_1^5}{5!} \\
%
h_{(5,6)} &=
  \frac{c_6 c_0^4}{1!4!} 
+ \frac{c_5 c_1 c_0^3}{1!1!3!} 
+ \frac{c_4 c_2 c_0^3}{1!1!3!}
+ \frac{c_4 c_1^2 c_0^2}{1!2!2!} 
+ \frac{c_3^2 c_0^3}{2!3!} 
+ \frac{c_3 c_2 c_1 c_0^2}{1!1!1!2!} 
+ \frac{c_3 c_1^3 c_0}{1!3!1!}
+ \frac{c_2^3 c_0^2}{3!2!} 
+ \frac{c_2^2 c_1^2 c_0}{2!2!1!} 
+ \frac{c_2 c_1^4}{1!4!} \\
%
&\ldots
\end{aligned} \right. \end{equation*}

\subsubsection{Показательная функция от многочлена}

\begin{equation*}
\begin{aligned}
C &= c_0 + c_1 x + c_2 x^2 + c_3 x^3 + c_4 x^4 + \ldots \\
\exp{C} &= \omega_{0}(C) + \omega_{1}(C) + \omega_{2}(C) + \ldots \\
\exp{C} &= h_0 + h_1 x + h_2 x^2 + h_3 x^3 + \ldots \\
\end{aligned}
\end{equation*}

\begin{equation*}
\left|
\begin{aligned}
h_0 &= \exp{c_0}
\\
h_1 
&= \left[\frac{c_1}{1!} \right] \exp{c_0}
\\ 
h_2 
&= \left[\frac{c_2}{1!} 
+ \frac{c_1^2}{2!} \right] \exp{c_0}
\\
h_3 
&= \left[\frac{c_3}{1!} 
+ \frac{c_2 c_1}{1!1!} 
+ \frac{c_1^3}{3!} \right] \exp{c_0}
\\
h_4 
&= \left[\frac{c_4}{1!} 
+ \frac{c_3 c_1}{1!1!} 
+ \frac{c_2^2}{2!} 
+ \frac{c_2 c_1^2}{1!2!} 
+ \frac{c_1^4}{4!} \right] \exp{c_0}
\\
h_5
&= \left[\frac{c_5}{1!}
+ \frac{c_4 c_1}{1!1!}
+ \frac{c_3 c_2}{1!1!}
+ \frac{c_3 c_1^2}{1!2!}
+ \frac{c_2^2 c_1}{2!1!}
+ \frac{c_2 c_1^3}{1!3!}
+ \frac{c_1^5}{5!} \right] \exp{c_0}
\\
&\ldots
\end{aligned}
\right.
\end{equation*}
