% !TeX root = ../Collection.tex

\section{Суммы значений функций}

\subsection{Степенные функции}

\begin{equation*}\begin{aligned}
(1 + x)^1 &=
  \frac{1!}{1!0!} 
+ \frac{1!}{0!1!} x
\\
(1 + x)^2 &= 
  \frac{2!}{2!0!} 
+ \frac{2!}{1!1!} x 
+ \frac{2!}{0!2!} x^2
\\
(1 + x)^3 &=
  \frac{3!}{3!0!} 
+ \frac{3!}{2!1!} x 
+ \frac{3!}{1!2!} x^2 
+ \frac{3!}{0!3!} x^3
\\
(1 + x)^4 &=
  \frac{4!}{4!0!} 
+ \frac{4!}{3!1!} x 
+ \frac{4!}{2!2!} x^2 
+ \frac{4!}{1!3!} x^3 
+ \frac{4!}{0!4!} x^4
\\
(1 + x)^5 &=
  \frac{5!}{5!0!} 
+ \frac{5!}{4!1!} x 
+ \frac{5!}{3!2!} x^2 
+ \frac{5!}{2!3!} x^3 
+ \frac{5!}{1!4!} x^4
+ \frac{5!}{0!5!} x^5
\\
&\ldots
\\
\end{aligned}\end{equation*}

\begin{equation*}\begin{aligned}
(x + 1)^0 - x^0 &= 0 \\
(x + 1)^1 - x^1 &= 1 \\
(x + 1)^2 - x^2 &= 1 + 2x \\
(x + 1)^3 - x^3 &= 1 + 3x + 3x^2 \\
\end{aligned}\end{equation*}

\subsection{$\omega_0$-функции}

\begin{equation*} \begin{aligned}
\phi_{(0,0)}(x) &=
  \frac{1^0}{0!} 
+ \frac{2^0}{0!} 
+ \frac{3^0}{0!} 
+ \frac{4^0}{0!} 
+ \ldots 
+ \frac{x^0}{0!} \\
%
\phi_{(0,1)}(x) &= 
  \frac{1^1}{1!} 
+ \frac{2^1}{1!} 
+ \frac{3^1}{1!} 
+ \frac{4^1}{1!} 
+ \ldots 
+ \frac{x^1}{1!} \\
%
\phi_{(0,2)}(x) &= 
  \frac{1^2}{2!} 
+ \frac{2^2}{2!} 
+ \frac{3^2}{2!} 
+ \frac{4^2}{2!} 
+ \ldots 
+ \frac{x^2}{2!} \\
%
\phi_{(0,3)}(x) &= 
  \frac{1^3}{3!} 
+ \frac{2^3}{3!} 
+ \frac{3^3}{3!} 
+ \frac{4^3}{3!} 
+ \ldots 
+ \frac{x^3}{3!} \\
%
&\ldots \\
\end{aligned} \end{equation*}

\begin{equation*} \begin{aligned}
\phi_{(0,0)}(x + 1) &= 
  \phi_{(0,0)}(x) + \omega_{(0,0)}(x + 1)
\\
\phi_{(0,1)}(x + 1) &= 
  \phi_{(0,1)}(x) + \omega_{(0,1)}(x + 1)  
\\
\phi_{(0,2)}(x + 1) &= 
  \phi_{(0,2)}(x) + \omega_{(0,2)}(x + 1)  
\\
\phi_{(0,3)}(x + 1) &= 
  \phi_{(0,3)}(x) + \omega_{(0,3)}(x + 1)  
\\
\phi_{(0,4)}(x + 1) &= 
  \phi_{(0,4)}(x) + \omega_{(0,4)}(x + 1)  
\\
&\ldots \\
\end{aligned} \end{equation*}

\begin{equation*} \begin{aligned}
\mathrm{D}_1 \left[\phi_{(0,0)}(x + 1) - \phi_{(0,0)}(x) \right] &= 0
\\
\mathrm{D}_1 \left[\phi_{(0,1)}(x + 1) - \phi_{(0,1)}(x) \right] &= \phi_{(0,0)}(x + 1) - \phi_{(0,0)}(x)  
\\
\mathrm{D}_1 \left[\phi_{(0,2)}(x + 1) - \phi_{(0,2)}(x) \right] &= \phi_{(0,1)}(x + 1) - \phi_{(0,1)}(x)  
\\
\mathrm{D}_1 \left[\phi_{(0,3)}(x + 1) - \phi_{(0,3)}(x) \right] &= \phi_{(0,2)}(x + 1) - \phi_{(0,2)}(x)  
\\
\mathrm{D}_1 \left[\phi_{(0,4)}(x + 1) - \phi_{(0,4)}(x) \right] &= \phi_{(0,3)}(x + 1) - \phi_{(0,3)}(x)  
\\
&\ldots \\
\end{aligned} \end{equation*}

\begin{equation*} \begin{aligned}
\mathrm{D}_1 \phi_{(0,0)}(x) &= t_0  
\\
\mathrm{D}_1 \phi_{(0,1)}(x) &= \phi_{(0,0)}(x) + t_1  
\\
\mathrm{D}_1 \phi_{(0,2)}(x) &= \phi_{(0,1)}(x) + t_2  
\\
\mathrm{D}_1 \phi_{(0,3)}(x) &= \phi_{(0,2)}(x) + t_3 
\\
\mathrm{D}_1 \phi_{(0,4)}(x) &= \phi_{(0,3)}(x) + t_4 
\\
&\ldots
\\
\end{aligned} \end{equation*}

\begin{equation*} \begin{aligned}
\phi_{(0,0)}(0) &= 0 & \phi_{(0,0)}(1) &= \omega_{(0,0)}(1)
\\
\phi_{(0,1)}(0) &= 0 & \phi_{(0,1)}(1) &= \omega_{(0,1)}(1)
\\
\phi_{(0,2)}(0) &= 0 & \phi_{(0,2)}(1) &= \omega_{(0,2)}(1)
\\
\phi_{(0,3)}(0) &= 0 & \phi_{(0,3)}(1) &= \omega_{(0,3)}(1)
\\
\phi_{(0,4)}(0) &= 0 & \phi_{(0,4)}(1) &= \omega_{(0,4)}(1)
\\
&\ldots & &\ldots
\\
\end{aligned} \end{equation*}

\begin{equation*} \begin{aligned}
\phi_{(0,0)}(x) &= 
  t_0 \frac{x}{1!} 
\\
\phi_{(0,1)}(x) &= 
  t_1 \frac{x}{1!} 
+ t_0 \frac{x^2}{2!} 
\\
\phi_{(0,2)}(x) &= 
  t_2 \frac{x}{1!} 
+ t_1 \frac{x^2}{2!} 
+ t_0 \frac{x^3}{3!} 
\\
\phi_{(0,3)}(x) &= 
  t_3 \frac{x}{1!} 
+ t_2 \frac{x^2}{2!} 
+ t_1 \frac{x^3}{3!} 
+ t_0 \frac{x^4}{4!} 
\\
&\ldots
\\
\end{aligned} \end{equation*}

\begin{equation*} \begin{aligned}
  t_0
+ t_1 x
+ t_2 x^2
+ t_3 x^3
+ \ldots
&
= \frac{x \exp{x}}{\exp{x} - 1}
= \frac{x}{2} \coth{\frac{x}{2}} 
+ \frac{x}{2}
\\
\end{aligned} \end{equation*}

\subsection{Производная}

\begin{equation*}
\begin{aligned}
T_1(x,a) &= 
  \frac{1!}{1!0!} f(x + a) 
- \frac{1!}{0!1!} f(x)
\\
T_2(x,a) &= 
  \frac{2!}{2!0!} f(x + 2 a) 
- \frac{2!}{1!1!} f(x + a) 
+ \frac{2!}{0!2!} f(x)
\\
T_3(x,a) &=
  \frac{3!}{3!0!} f(x + 3 a) 
- \frac{3!}{2!1!} f(x + 2 a) 
+ \frac{3!}{1!2!} f(x + a)
- \frac{3!}{0!3!} f(x)
\\
T_4(x,a) &= 
  \frac{4!}{4!0!} f(x + 4 a) 
- \frac{4!}{3!1!} f(x + 3 a) 
+ \frac{4!}{2!2!} f(x + 2 a) 
- \frac{4!}{1!3!} f(x + a) 
+ \frac{4!}{0!4!} f(x)
\\
&\ldots
\\
\end{aligned}
\end{equation*}

\begin{equation*}
\begin{aligned}
\mathrm{D}_1 f(x) &= \lim_{a \to 0} \frac{T_1(x,a)}{a} \\
%
\mathrm{D}_2 f(x) &= \lim_{a \to 0} \frac{T_2(x,a)}{a^2} \\
%
\mathrm{D}_3 f(x) &= \lim_{a \to 0} \frac{T_3(x,a)}{a^3} \\
%
\mathrm{D}_4 f(x) &= \lim_{a \to 0} \frac{T_4(x,a)}{a^4} \\
%
&\ldots \\
\end{aligned}
\end{equation*}

\begin{equation*}
\begin{aligned}
\mathrm{D}_{(1,0)} F(x, y) &=
\lim_{a \to 0}{\frac{
  F(x + a, y)
- F(x, y)
}{a}}
\\
\mathrm{D}_{(2,0)} F(x, y) &=
\lim_{a \to 0}{\frac{
  F(x + 2 a, y)
- 2 F(x + a, y)
+ F(x)
}{a^2}}
\\
\mathrm{D}_{(0,1)} F(x, y) &=
\lim_{a \to 0}{\frac{
  F(x, y + a)
- F(x, y)
}{a}}
\\
\mathrm{D}_{(1,1)} F(x, y) &=
\lim_{a \to 0}{\frac{{
  F(x + a, y + a)
- F(x, y + a)
- F(x + a, y)
+ F(x, y)
}}{a^2}}
\\
\end{aligned}
\end{equation*}
